Make function environments a parameter of assertions.

assertions.v
@@ -19,51 +19,52 @@ Local Hint Extern 1 (_ ⊆{_} _) => etransitivity; [|eassumption].
 
 (** * Definition of assertions *)
 Record assert (K : Set) `{Env K} := Assert {
-  assert_holds : env K → memenv K → stack K → nat → mem K → Prop;
-  assert_weaken Γ1 Γ2 Δ1 Δ2 ρ n n' m :
+  assert_holds : env K → memenv K → funenv K → stack K → nat → mem K → Prop;
+  assert_weaken Γ1 Γ2 Δ1 Δ2 δ1 δ2 ρ n n' m :
     ✓ Γ1 → ✓{Γ1,Δ1} m → ✓{Δ1}* ρ →
-    assert_holds Γ1 Δ1 ρ n m →
-    Γ1 ⊆ Γ2 → Δ1 ⇒ₘ Δ2 → n' ≤ n →
-    assert_holds Γ2 Δ2 ρ n' m
+    assert_holds Γ1 Δ1 δ1 ρ n m →
+    Γ1 ⊆ Γ2 → Δ1 ⇒ₘ Δ2 → δ1 ⊆ δ2 → n' ≤ n →
+    assert_holds Γ2 Δ2 δ2 ρ n' m
 }.
 Add Printing Constructor assert.
 
 Delimit Scope assert_scope with A.
 Bind Scope assert_scope with assert.
 Arguments Assert {_ _} _ _.
-Arguments assert_holds {_ _} _%A _ _ _ _ _.
-Arguments assert_weaken {_ _} _%A _ _ _ _ _ _ _ _ _ _ _ _ _ _ _.
+Arguments assert_holds {_ _} _%A _ _ _ _ _ _.
+Arguments assert_weaken {_ _} _%A _ _ _ _ _ _ _ _ _ _ _ _ _ _ _ _ _ _.
 
 (** The relation [P ⊆@{Γ} Q] states that the assertion [Q] is a logical
 consequence of [P] in [Γ] and [P ≡@{Γ} Q] states that [P] and [Q] are logically
 equivalent in [Γ]. *)
-Instance assert_entails `{Env K} : SubsetEqE (env K) (assert K) := λ Γ P Q,
-  ∀ Γ' Δ ρ n m,
-    Γ ⊆ Γ' → ✓ Γ' → ✓{Γ',Δ} m → ✓{Δ}* ρ →
-    assert_holds P Γ' Δ ρ n m → assert_holds Q Γ' Δ ρ n m.
-Instance assert_equiv `{Env K} : EquivE (env K) (assert K) := λ Γ P Q,
-  P ⊆{Γ} Q ∧ Q ⊆{Γ} P.
+Instance assert_entails `{Env K} :
+    SubsetEqE (env K * funenv K) (assert K) := λ Γδ P Q,
+  ∀ Γ Δ δ ρ n m,
+    Γδ.1 ⊆ Γ → ✓ Γ → Γδ.2 ⊆ δ → ✓{Γ,Δ} δ → ✓{Γ,Δ} m → ✓{Δ}* ρ →
+    assert_holds P Γ Δ δ ρ n m → assert_holds Q Γ Δ δ ρ n m.
+Instance assert_equiv `{Env K} :
+    EquivE (env K * funenv K) (assert K) := λ Γδ P Q, P ⊆{Γδ} Q ∧ Q ⊆{Γδ} P.
 
 (** * Hoare logic connectives *)
 (** Definitions and notations of the usual connectives of Hoare logic. *)
 Program Definition assert_False `{Env K} : assert K := {|
-  assert_holds Γ Δ ρ n m := False
+  assert_holds Γ Δ δ ρ n m := False
 |}.
 Next Obligation. naive_solver. Qed.
 Notation "'False'" := assert_False : assert_scope.
 Program Definition assert_True `{Env K} : assert K := {|
-  assert_holds Γ Δ ρ n m := True
+  assert_holds Γ Δ δ ρ n m := True
 |}.
 Next Obligation. naive_solver. Qed.
 Notation "'True'" := assert_True : assert_scope.
 
 Program Definition assert_impl `{Env K} (P Q : assert K) : assert K := {|
-  assert_holds Γ Δ ρ n m := ∀ Γ' Δ' n',
-    Γ ⊆ Γ' → ✓ Γ' → Δ ⇒ₘ Δ' → ✓{Γ',Δ'} m → n' ≤ n →
-    assert_holds P Γ' Δ' ρ n' m → assert_holds Q Γ' Δ' ρ n' m
+  assert_holds Γ Δ δ ρ n m := ∀ Γ' Δ' δ' n',
+    Γ ⊆ Γ' → ✓ Γ' → Δ ⇒ₘ Δ' → δ ⊆ δ' → ✓{Γ',Δ'} δ' → ✓{Γ',Δ'} m → n' ≤ n →
+    assert_holds P Γ' Δ' δ' ρ n' m → assert_holds Q Γ' Δ' δ' ρ n' m
 |}.
 Next Obligation.
-  intros ?? P Q Γ1 Γ2 Δ1 Δ2 ρ n n' m ??? HPQ ??? Γ3 Δ3 ???????.
+  intros ?? P Q Γ1 Γ2 Δ1 Δ2 δ1 δ2 ρ n1 n2 m ??? HPQ ???? Γ3 Δ3 δ3 n3 ????????.
   apply HPQ; eauto; lia.
 Qed.
 Infix "→" := assert_impl : assert_scope.
@@ -72,8 +73,8 @@ Notation "( P →)" := (assert_impl P) (only parsing) : assert_scope.
 Notation "(→ Q )" := (λ P, assert_impl P Q) (only parsing) : assert_scope.
 
 Program Definition assert_and `{Env K} (P Q : assert K) : assert K := {|
-  assert_holds Γ Δ ρ n m :=
-    assert_holds P Γ Δ ρ n m ∧ assert_holds Q Γ Δ ρ n m
+  assert_holds Γ Δ δ ρ n m :=
+    assert_holds P Γ Δ δ ρ n m ∧ assert_holds Q Γ Δ δ ρ n m
 |}.
 Next Obligation. naive_solver eauto using assert_weaken. Qed.
 Infix "∧" := assert_and : assert_scope.
@@ -82,8 +83,8 @@ Notation "( P ∧)" := (assert_and P) (only parsing) : assert_scope.
 Notation "(∧ Q )" := (λ P, assert_and P Q) (only parsing) : assert_scope.
 
 Program Definition assert_or `{Env K} (P Q : assert K) : assert K := {|
-  assert_holds Γ Δ ρ n m :=
-    assert_holds P Γ Δ ρ n m ∨ assert_holds Q Γ Δ ρ n m
+  assert_holds Γ Δ δ ρ n m :=
+    assert_holds P Γ Δ δ ρ n m ∨ assert_holds Q Γ Δ δ ρ n m
 |}.
 Next Obligation. naive_solver eauto using assert_weaken. Qed.
 Infix "∨" := assert_or : assert_scope.
@@ -101,25 +102,25 @@ Notation "( P ↔)" := (assert_iff P) (only parsing) : assert_scope.
 Notation "(↔ Q )" := (λ P, assert_iff P Q) (only parsing) : assert_scope.
 
 Program Definition assert_forall `{Env K} `(P: A → assert K) : assert K := {|
-  assert_holds := λ Γ Δ ρ n m, ∀ x, assert_holds (P x) Γ Δ ρ n m
+  assert_holds := λ Γ Δ δ ρ n m, ∀ x, assert_holds (P x) Γ Δ δ ρ n m
 |}.
 Next Obligation. naive_solver eauto using assert_weaken. Qed.
 Notation "∀ x .. y , P" :=
   (assert_forall (λ x, .. (assert_forall (λ y, P)) ..)) : assert_scope.
 
 Program Definition assert_exist `{Env K} `(P : A → assert K): assert K := {|
-  assert_holds := λ Γ Δ ρ n m, ∃ x, assert_holds (P x) Γ Δ ρ n m
+  assert_holds := λ Γ Δ δ ρ n m, ∃ x, assert_holds (P x) Γ Δ δ ρ n m
 |}.
 Next Obligation. naive_solver eauto using assert_weaken. Qed.
 Notation "∃ x .. y , P" :=
   (assert_exist (λ x, .. (assert_exist (λ y, P)) ..)) : assert_scope.
 
 Program Definition assert_later `{Env K} (P : assert K) : assert K := {|
-  assert_holds Γ Δ ρ n m := ∀ n', n' < n → assert_holds P Γ Δ ρ n' m
+  assert_holds Γ Δ δ ρ n m := ∀ n', n' < n → assert_holds P Γ Δ δ ρ n' m
 |}.
 Next Obligation.
-  intros ?? P Γ1 Γ2 Δ1 Δ2 ρ n n' m ??????? n'' ?.
-  eapply assert_weaken with _ _ n''; eauto with lia.
+  intros ?? P Γ1 Γ2 Δ1 Δ2 δ1 δ2 ρ n1 n2 m ???????? n3 ?.
+  eapply assert_weaken with _ _ _ n3; eauto with lia.
 Qed.
 Notation "▷ P" := (assert_later P) (at level 20) : assert_scope.
 
@@ -128,23 +129,23 @@ Notation "▷ P" := (assert_later P) (at level 20) : assert_scope.
 (called separating conjunction) asserts that the memory can be split into two
 disjoint parts such that [P] holds in the one part, and [Q] in the other. *)
 Program Definition assert_eq_mem `{Env K} (m : mem K) : assert K := {|
-  assert_holds Γ Δ ρ n m' := m' = m
+  assert_holds Γ Δ δ ρ n m' := m' = m
 |}.
 Next Obligation. naive_solver. Qed.
 Program Definition assert_Prop `{Env K} (P : Prop) : assert K := {|
-  assert_holds Γ Δ ρ n m := P ∧ m = ∅
+  assert_holds Γ Δ δ ρ n m := P ∧ m = ∅
 |}.
 Next Obligation. naive_solver. Qed.
 Notation "⌜ P ⌝" := (assert_Prop P) (format "⌜  P  ⌝") : assert_scope.
 Notation "'emp'" := (assert_Prop True) : assert_scope.
 
 Program Definition assert_sep `{EnvSpec K} (P Q : assert K) : assert K := {|
-  assert_holds Γ Δ ρ n m := ∃ m1 m2,
+  assert_holds Γ Δ δ ρ n m := ∃ m1 m2,
     m = m1 ∪ m2 ∧ ⊥[m1; m2] ∧
-    assert_holds P Γ Δ ρ n m1 ∧ assert_holds Q Γ Δ ρ n m2
+    assert_holds P Γ Δ δ ρ n m1 ∧ assert_holds Q Γ Δ δ ρ n m2
 |}.
 Next Obligation.
-  intros ??? P Q Γ1 Γ2 Δ1 Δ2 ρ n m ???? (m1&m2&->&?&?&?) ??.
+  intros ??? P Q Γ1 Γ2 Δ1 Δ2 δ1 δ2 ρ n m ???? (m1&m2&->&?&?&?) ????.
   eauto 15 using assert_weaken, cmap_valid_subseteq,
     @sep_union_subseteq_l, @sep_union_subseteq_r.
 Qed.
@@ -154,17 +155,17 @@ Notation "( P ★)" := (assert_sep P) (only parsing) : assert_scope.
 Notation "(★ Q )" := (λ P, assert_sep P Q) (only parsing) : assert_scope.
 
 Class MemExt `{EnvSpec K} (P : assert K) : Prop :=
-  mem_ext Γ : (P ★ True)%A ⊆{Γ} P.
+  mem_ext Γ δ : (P ★ True)%A ⊆{Γ,δ} P.
 Hint Extern 10 (MemExt _) => apply _.
 
 Program Definition assert_wand `{Env K} (P Q : assert K) : assert K := {|
-  assert_holds Γ Δ ρ n m2 := ∀ Γ' Δ' n' m1,
-    Γ ⊆ Γ' → ✓ Γ' → Δ ⇒ₘ Δ' → n' ≤ n →
+  assert_holds Γ Δ δ ρ n m2 := ∀ Γ' Δ' δ' n' m1,
+    Γ ⊆ Γ' → ✓ Γ' → Δ ⇒ₘ Δ' → δ ⊆ δ' → ✓{Γ',Δ'} δ' → n' ≤ n →
     ✓{Γ',Δ'} m1 → ✓{Γ',Δ'} m2 → ⊥[m1; m2] →
-    assert_holds P Γ' Δ' ρ n' m1 → assert_holds Q Γ' Δ' ρ n' (m1 ∪ m2)
+    assert_holds P Γ' Δ' δ' ρ n' m1 → assert_holds Q Γ' Δ' δ' ρ n' (m1 ∪ m2)
 |}.
 Next Obligation.
-  intros ?? P Q Γ1 Γ2 Δ1 Δ2 ρ n n' m ??? HPQ ??? Γ3 Δ3 ?????????.
+  intros ?? P Q Γ Γ2 Δ Δ2 δ1 δ2 ρ n n2 m ??? HPQ ???? Γ3 Δ3 δ3 n3 ???????????.
   apply HPQ; eauto; lia.
 Qed.
 Infix "-★" := assert_wand (at level 90) : assert_scope.
@@ -184,11 +185,11 @@ and [e ⇓ - : τlr] asserts that the expression [e] evaluates to an arbitrary
 value (in other words, [e] does not impose undefined behavior). *)
 Notation vassert K := (lrval K → assert K).
 Program Definition assert_expr `{EnvSpec K} (e : expr K) : vassert K := λ ν, {|
-  assert_holds Γ Δ ρ n m := ∃ τlr, (Γ,Δ,ρ.*2) ⊢ e : τlr ∧ ⟦ e ⟧ Γ ρ m = Some ν
+  assert_holds Γ Δ δ ρ n m := ∃ τlr, (Γ,Δ,ρ.*2) ⊢ e : τlr ∧ ⟦ e ⟧ Γ ρ m = Some ν
 |}.
 Next Obligation.
-  intros ??? e ν Γ1 Γ2 Δ1 Δ2 ρ n m ???? (τlr&?&?) ??; exists τlr; split;
-    eauto using expr_typed_weaken, expr_eval_weaken,
+  intros ??? e ν Γ1 Γ2 Δ1 Δ2 δ1 δ2 ρ n1 n2 m ??? (τlr&?&?) ??;
+    exists τlr; split; eauto using expr_typed_weaken, expr_eval_weaken,
     mem_lookup_weaken, mem_forced_weaken.
 Qed.
 Notation "e ⇓ ν" := (assert_expr e ν)%A
@@ -204,13 +205,13 @@ object at address [e1] with permission [x] and arbitrary contents. The Boolean
 Program Definition assert_singleton `{EnvSpec K}
     (e1 : expr K) (μ : bool) (γ : perm)
     (e2 : expr K) (τ : type K) : assert K := {|
-  assert_holds Γ Δ ρ n m := ∃ a v,
+  assert_holds Γ Δ δ ρ n m := ∃ a v,
     (Γ,Δ,ρ.*2) ⊢ e1 : inl τ ∧ ⟦ e1 ⟧ Γ ρ ∅ = Some (inl a) ∧
     (Γ,Δ,ρ.*2) ⊢ e2 : inr τ ∧ ⟦ e2 ⟧ Γ ρ ∅ = Some (inr v) ∧
     mem_singleton Γ Δ a μ γ v τ m
 |}.
 Next Obligation.
-  intros ??? e1 e2 ml γ τ Γ1 Γ2 Δ1 Δ2 ρ n m ???? (a&v&?&?&?&?&?) ??.
+  intros ??? e1 e2 ml γ τ Γ1 Γ2 Δ1 Δ2 δ1 δ2 ρ n1 n2 m ??? (a&v&?&?&?&?&?) ??.
   exists a v; split_ands; eauto using expr_typed_weaken,
     expr_eval_weaken_empty, mem_singleton_weaken, cmap_valid_memenv_valid.
 Qed.
@@ -225,14 +226,14 @@ Notation "e1 ↦{ μ , γ } - : τ" :=
 (** The assertion [P ◊] asserts that [P] holds if all sequenced locations
 are unlocked. *)
 Program Definition assert_unlock `{EnvSpec K} (P : assert K) : assert K := {|
-  assert_holds Γ Δ ρ n m := assert_holds P Γ Δ ρ n (mem_unlock_all m)
+  assert_holds Γ Δ δ ρ n m := assert_holds P Γ Δ δ ρ n (mem_unlock_all m)
 |}.
 Next Obligation.
   naive_solver eauto using assert_weaken, mem_unlock_all_valid.
 Qed.
 Notation "P ◊" := (assert_unlock P) (at level 20) : assert_scope.
 Class UnlockIndep `{EnvSpec K} (P : assert K) : Prop :=
-  unlock_indep Γ : P ⊆{Γ} (P ◊)%A.
+  unlock_indep Γ δ : P ⊆{Γ,δ} (P ◊)%A.
 Hint Extern 10 (UnlockIndep _) => apply _.
 
 (** To deal with block scope variables we need to lift an assertion such that
@@ -240,12 +241,12 @@ the De Bruijn indexes of its variables are increased. We define the lifting
 [P↑] of an assertion [P] semantically, and prove that it indeed behaves as
 expected. *)
 Program Definition assert_lift `{Env K} (P : assert K) : assert K := {|
-  assert_holds Γ Δ ρ n m := assert_holds P Γ Δ (tail ρ) n m
+  assert_holds Γ Δ δ ρ n m := assert_holds P Γ Δ δ (tail ρ) n m
 |}.
 Next Obligation. naive_solver eauto using assert_weaken, Forall_tail. Qed.
 Notation "P ↑" := (assert_lift P) (at level 20) : assert_scope.
 Class StackIndep `{Env K} (P : assert K) : Prop :=
-  stack_indep Γ : (P ↑)%A ≡{Γ} P.
+  stack_indep Γ δ : (P ↑)%A ≡{Γ,δ} P.
 Hint Extern 10 (StackIndep _) => apply _.
 
 Section assertions.
@@ -268,291 +269,299 @@ Ltac solve t :=
   | progress autounfold with assert in *];
   naive_solver t.
 
+Lemma assert_entails_spec P Q Γ Δ δ ρ n m :
+  ✓ Γ → ✓{Γ,Δ} δ → ✓{Γ,Δ} m → ✓{Δ}* ρ →
+  P ⊆{Γ,δ} Q → assert_holds P Γ Δ δ ρ n m → assert_holds Q Γ Δ δ ρ n m.
+Proof. intros ???? HPQ; apply HPQ; auto. Qed.
+
 (** Ordinary logic connections *)
-Global Instance: PreOrder (⊆{Γ}).
+Global Instance: PreOrder (⊆{Γ,δ}).
 Proof. split; solve eauto. Qed.
-Global Instance: Equivalence (≡{Γ}).
+Global Instance: Equivalence (≡{Γ,δ}).
 Proof. split; red; solve eauto. Qed.
-Global Instance: Proper ((≡{Γ}) ==> (≡{Γ}) ==> iff) (⊆{Γ}).
+Global Instance: Proper ((≡{Γ,δ}) ==> (≡{Γ,δ}) ==> iff) (⊆{Γ,δ}).
 Proof. solve eauto. Qed.
-Global Instance: Proper (flip (⊆{Γ}) ==> (⊆{Γ}) ==> (⊆{Γ})) (→)%A.
+Global Instance: Proper (flip (⊆{Γ,δ}) ==> (⊆{Γ,δ}) ==> (⊆{Γ,δ})) (→)%A.
 Proof.
-  intros Γ1 P1 P2 HP Q1 Q2 HQ Γ2 Δ ρ n m ???? HPQ Γ3 Δ2 n2 ????? HP2.
-  eapply HQ; eauto using indexes_valid_weaken.
+  intros Γ1 δ1 P1 P2 HP Q1 Q2 HQ Γ2 Δ1 δ2 ρ n m ?????? HPQ Γ3 Δ2 δ3 n2 ????????.
+  eapply HQ; eauto 8 using indexes_valid_weaken.
 Qed.
-Global Instance: Proper ((≡{Γ}) ==> (≡{Γ}) ==> (≡{Γ})) (→)%A.
-Proof. by intros ??? [??] ?? [??]; split; f_equiv. Qed.
-Global Instance: Proper ((≡{Γ}) ==> (≡{Γ}) ==> (≡{Γ})) (∧)%A.
+Global Instance: Proper ((≡{Γ,δ}) ==> (≡{Γ,δ}) ==> (≡{Γ,δ})) (→)%A.
+Proof. by intros ???? [??] ?? [??]; split; f_equiv. Qed.
+Global Instance: Proper ((≡{Γ,δ}) ==> (≡{Γ,δ}) ==> (≡{Γ,δ})) (∧)%A.
 Proof. solve eauto. Qed.
-Global Instance: Proper ((⊆{Γ}) ==> (⊆{Γ}) ==> (⊆{Γ})) (∧)%A.
+Global Instance: Proper ((⊆{Γ,δ}) ==> (⊆{Γ,δ}) ==> (⊆{Γ,δ})) (∧)%A.
 Proof. solve eauto. Qed.
-Global Instance: Proper ((≡{Γ}) ==> (≡{Γ}) ==> (≡{Γ})) (∨)%A.
+Global Instance: Proper ((≡{Γ,δ}) ==> (≡{Γ,δ}) ==> (≡{Γ,δ})) (∨)%A.
 Proof. solve eauto. Qed.
-Global Instance: Proper ((⊆{Γ}) ==> (⊆{Γ}) ==> (⊆{Γ})) (∨)%A.
+Global Instance: Proper ((⊆{Γ,δ}) ==> (⊆{Γ,δ}) ==> (⊆{Γ,δ})) (∨)%A.
 Proof. solve eauto. Qed.
-Global Instance: Proper ((≡{Γ}) ==> (≡{Γ}) ==> (≡{Γ})) (↔)%A.
-Proof. by intros ???????; unfold assert_iff; do 2 f_equiv. Qed.
-Global Instance: Proper ((≡{Γ}) ==> (≡{Γ})) assert_not.
-Proof. by intros ????; unfold assert_not; f_equiv. Qed.
-Global Instance: Proper (flip (⊆{Γ}) ==> (⊆{Γ})) assert_not.
-Proof. by intros ????; unfold assert_not; f_equiv. Qed.
+Global Instance: Proper ((≡{Γ,δ}) ==> (≡{Γ,δ}) ==> (≡{Γ,δ})) (↔)%A.
+Proof. by intros ????????; unfold assert_iff; do 2 f_equiv. Qed.
+Global Instance: Proper ((≡{Γ,δ}) ==> (≡{Γ,δ})) assert_not.
+Proof. by intros ?????; unfold assert_not; f_equiv. Qed.
+Global Instance: Proper (flip (⊆{Γ,δ}) ==> (⊆{Γ,δ})) assert_not.
+Proof. by intros ?????; unfold assert_not; f_equiv. Qed.
 Global Instance:
-  Proper (pointwise_relation _ (≡{Γ}) ==> (≡{Γ})) (@assert_forall _ _ A).
-Proof. solve eauto. Qed.
-Global Instance:
-  Proper (pointwise_relation _ (⊆{Γ}) ==> (⊆{Γ})) (@assert_forall _ _ A).
+  Proper (pointwise_relation _ (≡{Γ,δ}) ==> (≡{Γ,δ})) (@assert_forall _ _ A).
 Proof. solve eauto. Qed.
 Global Instance:
-  Proper (pointwise_relation _ (≡{Γ}) ==> (≡{Γ})) (@assert_exist _ _ A).
+  Proper (pointwise_relation _ (⊆{Γ,δ}) ==> (⊆{Γ,δ})) (@assert_forall _ _ A).
 Proof. solve eauto. Qed.
 Global Instance:
-  Proper (pointwise_relation _ (⊆{Γ}) ==> (⊆{Γ})) (@assert_exist _ _ A).
+  Proper (pointwise_relation _ (≡{Γ,δ}) ==> (≡{Γ,δ})) (@assert_exist _ _ A).
 Proof. solve eauto. Qed.
 Global Instance:
-  Proper (pointwise_relation _ (flip (⊆{Γ})) ==> (flip (⊆{Γ})))
+  Proper (pointwise_relation _ (⊆{Γ,δ}) ==> (⊆{Γ,δ})) (@assert_exist _ _ A).
+Proof. solve eauto. Qed.
+Global Instance:
+  Proper (pointwise_relation _ (flip (⊆{Γ,δ})) ==> (flip (⊆{Γ,δ})))
   (@assert_exist _ _ A).
 Proof. solve eauto. Qed.
 
-Global Instance: Commutative (≡{Γ}) (↔)%A.
+Global Instance: Commutative (≡{Γ,δ}) (↔)%A.
 Proof. red; solve eauto. Qed.
-Global Instance: Commutative (≡{Γ}) (∧)%A.
+Global Instance: Commutative (≡{Γ,δ}) (∧)%A.
 Proof. red; solve eauto. Qed.
-Global Instance: Associative (≡{Γ}) (∧)%A.
+Global Instance: Associative (≡{Γ,δ}) (∧)%A.
 Proof. red; solve eauto. Qed.
-Global Instance: Idempotent (≡{Γ}) (∧)%A.
+Global Instance: Idempotent (≡{Γ,δ}) (∧)%A.
 Proof. red; solve eauto. Qed.
-Global Instance: LeftId (≡{Γ}) True%A (∧)%A.
+Global Instance: LeftId (≡{Γ,δ}) True%A (∧)%A.
 Proof. red; solve eauto. Qed.
-Global Instance: RightId (≡{Γ}) True%A (∧)%A.
+Global Instance: RightId (≡{Γ,δ}) True%A (∧)%A.
 Proof. red; solve eauto. Qed.
-Global Instance: LeftAbsorb (≡{Γ}) False%A (∧)%A.
+Global Instance: LeftAbsorb (≡{Γ,δ}) False%A (∧)%A.
 Proof. red; solve eauto. Qed.
-Global Instance: RightAbsorb (≡{Γ}) False%A (∧)%A.
+Global Instance: RightAbsorb (≡{Γ,δ}) False%A (∧)%A.
 Proof. red; solve eauto. Qed.
-Global Instance: Commutative (≡{Γ}) (∨)%A.
+Global Instance: Commutative (≡{Γ,δ}) (∨)%A.
 Proof. red; solve eauto. Qed.
-Global Instance: Associative (≡{Γ}) (∨)%A.
+Global Instance: Associative (≡{Γ,δ}) (∨)%A.
 Proof. red; solve eauto. Qed.
-Global Instance: Idempotent (≡{Γ}) (∨)%A.
+Global Instance: Idempotent (≡{Γ,δ}) (∨)%A.
 Proof. red; solve eauto. Qed.
-Global Instance: LeftId (≡{Γ}) False%A (∨)%A.
+Global Instance: LeftId (≡{Γ,δ}) False%A (∨)%A.
 Proof. red; solve eauto. Qed.
-Global Instance: RightId (≡{Γ}) False%A (∨)%A.
+Global Instance: RightId (≡{Γ,δ}) False%A (∨)%A.
 Proof. red; solve eauto. Qed.
-Global Instance: LeftAbsorb (≡{Γ}) True%A (∨)%A.
+Global Instance: LeftAbsorb (≡{Γ,δ}) True%A (∨)%A.
 Proof. red; solve eauto. Qed.
-Global Instance: RightAbsorb (≡{Γ}) True%A (∨)%A.
+Global Instance: RightAbsorb (≡{Γ,δ}) True%A (∨)%A.
 Proof. red; solve eauto. Qed.
-Lemma assert_False_elim Γ P : False%A ⊆{Γ} P.
+Lemma assert_False_elim Γ δ P : False%A ⊆{Γ,δ} P.
 Proof. solve eauto. Qed.
-Lemma assert_True_intro Γ P : P ⊆{Γ} True%A.
+Lemma assert_True_intro Γ δ P : P ⊆{Γ,δ} True%A.
 Proof. solve eauto. Qed.
-Lemma assert_and_l Γ P Q : (P ∧ Q)%A ⊆{Γ} P.
+Lemma assert_and_l Γ δ P Q : (P ∧ Q)%A ⊆{Γ,δ} P.
 Proof. solve eauto. Qed.
-Lemma assert_and_r Γ P Q : (P ∧ Q)%A ⊆{Γ} Q.
+Lemma assert_and_r Γ δ P Q : (P ∧ Q)%A ⊆{Γ,δ} Q.
 Proof. solve eauto. Qed.
-Lemma assert_impl_and Γ P Q : P ⊆{Γ} Q → P ≡{Γ} (P ∧ Q)%A.
+Lemma assert_impl_and Γ δ P Q : P ⊆{Γ,δ} Q → P ≡{Γ,δ} (P ∧ Q)%A.
 Proof. solve eauto. Qed.
-Lemma assert_and_intro Γ P Q1 Q2 : P ⊆{Γ} Q1 → P ⊆{Γ} Q2 → P ⊆{Γ} (Q1 ∧ Q2)%A.
+Lemma assert_and_intro Γ δ P Q1 Q2 :
+  P ⊆{Γ,δ} Q1 → P ⊆{Γ,δ} Q2 → P ⊆{Γ,δ} (Q1 ∧ Q2)%A.
 Proof. solve eauto. Qed.
-Lemma assert_and_elim_l Γ P1 P2 Q : P1 ⊆{Γ} Q → (P1 ∧ P2)%A ⊆{Γ} Q.
+Lemma assert_and_elim_l Γ δ P1 P2 Q : P1 ⊆{Γ,δ} Q → (P1 ∧ P2)%A ⊆{Γ,δ} Q.
 Proof. solve eauto. Qed.
-Lemma assert_and_elim_r Γ P1 P2 Q : P2 ⊆{Γ} Q → (P1 ∧ P2)%A ⊆{Γ} Q.
+Lemma assert_and_elim_r Γ δ P1 P2 Q : P2 ⊆{Γ,δ} Q → (P1 ∧ P2)%A ⊆{Γ,δ} Q.
 Proof. solve eauto. Qed.
-Lemma assert_or_l Γ P Q : P ⊆{Γ} (P ∨ Q)%A.
+Lemma assert_or_l Γ δ P Q : P ⊆{Γ,δ} (P ∨ Q)%A.
 Proof. solve eauto. Qed.
-Lemma assert_or_r Γ P Q : Q ⊆{Γ} (P ∨ Q)%A.
+Lemma assert_or_r Γ δ P Q : Q ⊆{Γ,δ} (P ∨ Q)%A.
 Proof. solve eauto. Qed.
-Lemma assert_forall_intro {A} Γ P (Q : A → assert K) :
-  (∀ x, P ⊆{Γ} Q x) → P ⊆{Γ} (∀ x, Q x)%A.
+Lemma assert_forall_intro {A} Γ δ P (Q : A → assert K) :
+  (∀ x, P ⊆{Γ,δ} Q x) → P ⊆{Γ,δ} (∀ x, Q x)%A.
 Proof. solve eauto. Qed.
-Lemma assert_forall_elim {A} Γ (P : A → assert K) Q x :
-  (P x ⊆{Γ} Q) → (∀ x, P x)%A ⊆{Γ} Q.
+Lemma assert_forall_elim {A} Γ δ (P : A → assert K) Q x :
+  (P x ⊆{Γ,δ} Q) → (∀ x, P x)%A ⊆{Γ,δ} Q.
 Proof. solve eauto. Qed.
-Lemma assert_exist_intro {A} Γ P (Q : A → assert K) x :
-  P ⊆{Γ} Q x → P ⊆{Γ} (∃ x, Q x)%A.
+Lemma assert_exist_intro {A} Γ δ P (Q : A → assert K) x :
+  P ⊆{Γ,δ} Q x → P ⊆{Γ,δ} (∃ x, Q x)%A.
 Proof. solve eauto. Qed.
-Lemma assert_exist_elim {A} Γ (P : A → assert K) Q :
-  (∀ x, P x ⊆{Γ} Q) → (∃ x, P x)%A ⊆{Γ} Q.
+Lemma assert_exist_elim {A} Γ δ (P : A → assert K) Q :
+  (∀ x, P x ⊆{Γ,δ} Q) → (∃ x, P x)%A ⊆{Γ,δ} Q.
 Proof. solve eauto. Qed.
-Lemma assert_and_exist {A} Γ P (Q : A → assert K) :
-  (P ∧ ∃ x, Q x)%A ≡{Γ} (∃ x, P ∧ Q x)%A.
+Lemma assert_and_exist {A} Γ δ P (Q : A → assert K) :
+  (P ∧ ∃ x, Q x)%A ≡{Γ,δ} (∃ x, P ∧ Q x)%A.
 Proof. solve eauto. Qed.
-Lemma assert_exist_and {A} Γ (P : A → assert K) Q :
-  ((∃ x, P x) ∧ Q)%A ≡{Γ} (∃ x, P x ∧ Q)%A.
+Lemma assert_exist_and {A} Γ δ (P : A → assert K) Q :
+  ((∃ x, P x) ∧ Q)%A ≡{Γ,δ} (∃ x, P x ∧ Q)%A.
 Proof. solve eauto. Qed.
-Lemma assert_exist_exist {A B} Γ (P : A → B → assert K) :
-  (∃ x y, P x y)%A ≡{Γ} (∃ y x, P x y)%A.
+Lemma assert_exist_exist {A B} Γ δ (P : A → B → assert K) :
+  (∃ x y, P x y)%A ≡{Γ,δ} (∃ y x, P x y)%A.
 Proof. solve eauto. Qed.
 
 (** Later *)
-Lemma assert_later_lob Γ P : (▷P → P)%A ⊆{Γ} P.
+Lemma assert_later_lob Γ δ P : (▷P → P)%A ⊆{Γ,δ} P.
 Proof.
-  intros Γ1 Δ ρ n m ???? HP; induction n as [|n IH].
+  intros Γ1 Δ δ1 ρ n m ?????? HP; induction n as [|n IH].
   { apply HP; eauto. intros n'; lia. }
   eapply HP; eauto. intros n' ?.
-  eapply assert_weaken with _ _ n; eauto with lia.
-  eapply IH, assert_weaken with _ _ (S n); eauto with lia.
+  eapply assert_weaken with _ _ δ1 n; eauto with lia.
+  eapply IH, assert_weaken with _ _ _ (S n); eauto with lia.
 Qed.
-Lemma assert_later_weaken Γ P : P ⊆{Γ} (▷P)%A.
+Lemma assert_later_weaken Γ δ P : P ⊆{Γ,δ} (▷P)%A.
 Proof.
-  intros Γ1 Δ ρ n m ????? n' ?.
-  eapply assert_weaken with _ _ n; eauto with lia.
+  intros Γ1 Δ ρ δ1 n m ??????? n' ?.
+  eapply assert_weaken with _ _ _ n; eauto with lia.
 Qed.
-Lemma assert_later_impl Γ P Q : (▷(P → Q))%A ⊆{Γ} (▷P → ▷Q)%A.
+Lemma assert_later_impl Γ δ P Q : (▷(P → Q))%A ⊆{Γ,δ} (▷P → ▷Q)%A.
 Proof.
-  intros Γ1 Δ1 ρ n m ???? HPQ Γ2 Δ2 n' ?????? n'' ?.
+  intros Γ1 Δ1 δ1 ρ n1 m ?????? HPQ Γ2 Δ2 δ2 n2 ???????? n3 ?.
   eapply HPQ; eauto; lia.
 Qed.
-Lemma assert_later_and Γ P Q : (▷(P ∧ Q))%A ≡{Γ} (▷P ∧ ▷Q)%A.
+Lemma assert_later_and Γ δ P Q : (▷(P ∧ Q))%A ≡{Γ,δ} (▷P ∧ ▷Q)%A.
 Proof. solve eauto. Qed.
-Lemma assert_later_or Γ P Q : (▷P ∨ ▷Q)%A ⊆{Γ} (▷(P ∨ Q))%A.
+Lemma assert_later_or Γ δ P Q : (▷P ∨ ▷Q)%A ⊆{Γ,δ} (▷(P ∨ Q))%A.
 Proof. solve eauto. Qed.
-Lemma assert_later_forall {A} Γ (P : A → assert K) :
-  (▷(∀ x, P x))%A ≡{Γ} (∀ x, ▷(P x))%A.
+Lemma assert_later_forall {A} Γ δ (P : A → assert K) :
+  (▷(∀ x, P x))%A ≡{Γ,δ} (∀ x, ▷(P x))%A.
 Proof. solve eauto. Qed.
-Lemma assert_later_exists {A} Γ (P : A → assert K) :
-  (∃ x, ▷(P x))%A ⊆{Γ} (▷(∃ x, P x))%A.
+Lemma assert_later_exists {A} Γ δ (P : A → assert K) :
+  (∃ x, ▷(P x))%A ⊆{Γ,δ} (▷(∃ x, P x))%A.
 Proof. solve eauto. Qed.
 
 (** Separation logic connectives *)
-Global Instance: Proper (impl ==> (⊆{Γ})) assert_Prop.
+Global Instance: Proper (impl ==> (⊆{Γ,δ})) assert_Prop.
 Proof. solve eauto. Qed.
-Global Instance: Proper (iff ==> (≡{Γ})) assert_Prop.
+Global Instance: Proper (iff ==> (≡{Γ,δ})) assert_Prop.
 Proof. solve eauto. Qed.
-Global Instance: Proper ((⊆{Γ}) ==> (⊆{Γ}) ==> (⊆{Γ})) (★)%A.
+Global Instance: Proper ((⊆{Γ,δ}) ==> (⊆{Γ,δ}) ==> (⊆{Γ,δ})) (★)%A.
 Proof.
   solve ltac:(eauto 15 using cmap_valid_subseteq,
     @sep_union_subseteq_l, @sep_union_subseteq_r).
 Qed.
-Global Instance: Proper (flip (⊆{Γ}) ==> flip (⊆{Γ}) ==> flip (⊆{Γ})) (★)%A.
+Global Instance:
+  Proper (flip (⊆{Γ,δ}) ==> flip (⊆{Γ,δ}) ==> flip (⊆{Γ,δ})) (★)%A.
 Proof.
   solve ltac:(eauto 15 using cmap_valid_subseteq,
     @sep_union_subseteq_l, @sep_union_subseteq_r).
 Qed.
-Global Instance: Proper ((≡{Γ}) ==> (≡{Γ}) ==> (≡{Γ})) (★)%A.
+Global Instance: Proper ((≡{Γ,δ}) ==> (≡{Γ,δ}) ==> (≡{Γ,δ})) (★)%A.
 Proof.
-  by intros ??? [??] ?? [??]; split;
-    apply (_ : Proper ((⊆{Γ}) ==> (⊆{Γ}) ==> (⊆{Γ})) (★)%A).
+  by intros ???? [??] ?? [??]; split;
+    apply (_ : Proper ((⊆{Γ,δ}) ==> (⊆{Γ,δ}) ==> (⊆{Γ,δ})) (★)%A).
 Qed.
-Global Instance: Proper (Forall2 (≡{Γ}) ==> (≡{Γ})) assert_sep_list.
+Global Instance: Proper (Forall2 (≡{Γ,δ}) ==> (≡{Γ,δ})) assert_sep_list.
 Proof.
   induction 1; simpl; [done|];
-    by apply (_ : Proper ((≡{Γ}) ==> (≡{Γ}) ==> (≡{Γ})) (★)%A).
+    by apply (_ : Proper ((≡{Γ,δ}) ==> (≡{Γ,δ}) ==> (≡{Γ,δ})) (★)%A).
 Qed.
-Global Instance: Proper (flip (⊆{Γ}) ==> (⊆{Γ}) ==> (⊆{Γ})) (-★)%A.
+Global Instance: Proper (flip (⊆{Γ,δ}) ==> (⊆{Γ,δ}) ==> (⊆{Γ,δ})) (-★)%A.
 Proof.
-  intros Γ1 P1 P2 HP Q1 Q2 HQ Γ2 Δ ρ n m ???? HPQ Γ3 Δ2 m2 n2 ??????? HP2.
-  apply HQ; eauto using indexes_valid_weaken, cmap_union_valid_2.
+  intros Γ1 δ1 P1 P2 HP Q1 Q2 HQ Γ2 Δ1 δ2 ρ n1 m
+    ?????? HPQ Γ3 Δ2 δ3 n2 ???????????.
+  apply HQ; eauto 10 using indexes_valid_weaken, cmap_union_valid_2.
 Qed.
-Global Instance: Proper ((≡{Γ}) ==> (≡{Γ}) ==> (≡{Γ})) (-★)%A.
+Global Instance: Proper ((≡{Γ,δ}) ==> (≡{Γ,δ}) ==> (≡{Γ,δ})) (-★)%A.
 Proof.
-  by intros ??? [??] ?? [??]; split;
-    apply (_ : Proper (flip (⊆{Γ}) ==> (⊆{Γ}) ==> (⊆{Γ})) (-★)%A).
+  by intros ???? [??] ?? [??]; split;
+    apply (_ : Proper (flip (⊆{Γ,δ}) ==> (⊆{Γ,δ}) ==> (⊆{Γ,δ})) (-★)%A).
 Qed.
 
-Global Instance: Commutative (⊆{Γ}) (★)%A.
+Global Instance: Commutative (⊆{Γ,δ}) (★)%A.
 Proof.
-  intros Γ P Q Γ1 Δ1 ρ n m ???? (m1&m2&->&?&?&?).
+  intros Γ δ P Q Γ1 Δ δ1 ρ n m ?????? (m1&m2&->&?&?&?).
   exists m2 m1. rewrite sep_commutative by auto; auto.
 Qed.
-Global Instance: Commutative (≡{Γ}) (★)%A.
+Global Instance: Commutative (≡{Γ,δ}) (★)%A.
 Proof. split; by rewrite (commutative (★)%A). Qed.
-Global Instance: LeftId (≡{Γ}) emp%A (★)%A.
+Global Instance: LeftId (≡{Γ,δ}) emp%A (★)%A.
 Proof.
-  intros Γ; intros P; split.
-  * intros Γ1 Δ1 ρ n m ???? (m1&m2&->&?&[_ ->]&?).
+  intros δ Γ; intros P; split.
+  * intros Γ1 Δ δ1 ρ n m ?????? (m1&m2&->&?&[_ ->]&?).
     rewrite sep_left_id by auto; auto.
-  * intros Γ1 Δ1 ρ n m ?????. eexists ∅, m.
+  * intros Γ1 Δ δ1 ρ n m ???????. eexists ∅, m.
     rewrite sep_left_id, sep_disjoint_equiv_empty,
       sep_disjoint_list_singleton by eauto; solve eauto.
 Qed.
-Global Instance: RightId (≡{Γ}) emp%A (★)%A.
-Proof. intros ??. by rewrite (commutative _), (left_id _ _). Qed.
-Global Instance: LeftAbsorb (≡{Γ}) False%A (★)%A.
+Global Instance: RightId (≡{Γ,δ}) emp%A (★)%A.
+Proof. intros ???. by rewrite (commutative _), (left_id _ _). Qed.
+Global Instance: LeftAbsorb (≡{Γ,δ}) False%A (★)%A.
 Proof. red; solve eauto. Qed.
-Global Instance: RightAbsorb (≡{Γ}) False%A (★)%A.
+Global Instance: RightAbsorb (≡{Γ,δ}) False%A (★)%A.
 Proof. red; solve eauto. Qed.
-Global Instance: Associative (≡{Γ}) (★)%A.
+Global Instance: Associative (≡{Γ,δ}) (★)%A.
 Proof.
-  intros Γ. assert (∀ P Q R, ((P ★ Q) ★ R)%A ⊆{Γ} (P ★ (Q ★ R))%A).
-  { intros P Q R Γ1 Δ1 ρ ? n ???? (?&m3&->&?&(m1&m2&->&?&?&?)&?).
+  intros Γ δ. assert (∀ P Q R, ((P ★ Q) ★ R)%A ⊆{Γ,δ} (P ★ (Q ★ R))%A).
+  { intros P Q R Γ1 Δ δ1 ρ ? n ?????? (?&m3&->&?&(m1&m2&->&?&?&?)&?).
     exists m1 (m2 ∪ m3); rewrite sep_associative by auto; split_ands; auto.
     exists m2 m3; auto. }
-  assert (∀ P Q R, (P ★ (Q ★ R))%A ⊆{Γ} ((P ★ Q) ★ R)%A).
-  { intros P Q R Γ1 Δ1 ρ ? n ???? (m1&?&->&?&?&(m2&m3&->&?&?&?)).
+  assert (∀ P Q R, (P ★ (Q ★ R))%A ⊆{Γ,δ} ((P ★ Q) ★ R)%A).
+  { intros P Q R Γ1 Δ δ1 ρ ? n ?????? (m1&?&->&?&?&(m2&m3&->&?&?&?)).
     exists (m1 ∪ m2) m3; rewrite sep_associative by auto; split_ands; auto.
     exists m1 m2; auto. }
   split; auto.
 Qed.
 
-Lemma assert_Prop_impl Γ (P Q : Prop) : ⌜ P → Q ⌝%A ⊆{Γ} (⌜P⌝ → ⌜Q⌝)%A.
+Lemma assert_Prop_impl Γ δ (P Q : Prop) : ⌜ P → Q ⌝%A ⊆{Γ,δ} (⌜P⌝ → ⌜Q⌝)%A.
 Proof. solve eauto. Qed.
-Lemma assert_Prop_not Γ (P : Prop) : ⌜ ¬P ⌝%A ⊆{Γ} (¬⌜P⌝)%A.
+Lemma assert_Prop_not Γ δ (P : Prop) : ⌜ ¬P ⌝%A ⊆{Γ,δ} (¬⌜P⌝)%A.
 Proof. solve eauto. Qed.
-Lemma assert_Prop_and Γ (P Q : Prop) : ⌜ P ∧ Q ⌝%A ≡{Γ} (⌜P⌝ ∧ ⌜Q⌝)%A.
+Lemma assert_Prop_and Γ δ (P Q : Prop) : ⌜ P ∧ Q ⌝%A ≡{Γ,δ} (⌜P⌝ ∧ ⌜Q⌝)%A.
 Proof. solve eauto. Qed.
-Lemma assert_Prop_or Γ (P Q : Prop) : ⌜ P ∨ Q ⌝%A ≡{Γ} (⌜P⌝ ∨ ⌜Q⌝)%A.
+Lemma assert_Prop_or Γ δ (P Q : Prop) : ⌜ P ∨ Q ⌝%A ≡{Γ,δ} (⌜P⌝ ∨ ⌜Q⌝)%A.
 Proof. solve eauto. Qed.
-Lemma assert_Prop_l Γ (P : Prop) Q : P → (⌜ P ⌝ ★ Q)%A ≡{Γ} Q.
+Lemma assert_Prop_l Γ δ (P : Prop) Q : P → (⌜ P ⌝ ★ Q)%A ≡{Γ,δ} Q.
 Proof.
   intros. assert (P ↔ True) as -> by (by split; intros _).
   by rewrite (left_id emp%A _).
 Qed.
-Lemma assert_Prop_r Γ (P : Prop) Q : P → (Q ★ ⌜ P ⌝)%A ≡{Γ} Q.
+Lemma assert_Prop_r Γ δ (P : Prop) Q : P → (Q ★ ⌜ P ⌝)%A ≡{Γ,δ} Q.
 Proof. intros. by rewrite (commutative (★))%A, assert_Prop_l. Qed.
-Lemma assert_Prop_intro_l Γ (P : Prop) Q R :
-  (P → Q ⊆{Γ} R) → (⌜ P ⌝ ★ Q)%A ⊆{Γ} R.
+Lemma assert_Prop_intro_l Γ δ (P : Prop) Q R :
+  (P → Q ⊆{Γ,δ} R) → (⌜ P ⌝ ★ Q)%A ⊆{Γ,δ} R.
 Proof.
-  intros HQR Γ1 Δ1 ρ n ??? Hm ? (m1&m2&->&?&[? ->]&?).
+  intros HQR Γ1 Δ δ1 ρ n ????? Hm ? (m1&m2&->&?&[? ->]&?).
   rewrite sep_left_id in Hm |- * by auto; by apply HQR.
 Qed.
-Lemma assert_Prop_intro_r Γ (P : Prop) Q R :
-  (P → Q ⊆{Γ} R) → (Q ★ ⌜ P ⌝)%A ⊆{Γ} R.
+Lemma assert_Prop_intro_r Γ δ (P : Prop) Q R :
+  (P → Q ⊆{Γ,δ} R) → (Q ★ ⌜ P ⌝)%A ⊆{Γ,δ} R.
 Proof. rewrite (commutative (★)%A). by apply assert_Prop_intro_l. Qed.
-Lemma assert_Prop_True Γ P (Q : Prop) :
-  P ⊆{Γ} (⌜ Q ⌝ ★ True)%A → P ⊆{Γ} (⌜ Q ⌝ ★ P)%A.
+Lemma assert_Prop_True Γ δ P (Q : Prop) :
+  P ⊆{Γ,δ} (⌜ Q ⌝ ★ True)%A → P ⊆{Γ,δ} (⌜ Q ⌝ ★ P)%A.
 Proof.
-  intros HPQ Γ' Δ ρ n m ???? HP.
-  destruct (HPQ Γ' Δ ρ n m) as (m1&m2&->&?&[? ->]&?); auto.
+  intros HPQ Γ1 Δ δ1 ρ n m ?????? HP.
+  destruct (HPQ Γ1 Δ δ1 ρ n m) as (m1&m2&->&?&[? ->]&?); auto.
   rewrite sep_left_id in HP by auto; solve eauto.
 Qed.
 
-Lemma assert_sep_preserving Γ P P' Q Q' :
-  P ⊆{Γ} P' → Q ⊆{Γ} Q' → (P ★ Q)%A ⊆{Γ} (P' ★ Q')%A.
+Lemma assert_sep_preserving Γ δ P P' Q Q' :
+  P ⊆{Γ,δ} P' → Q ⊆{Γ,δ} Q' → (P ★ Q)%A ⊆{Γ,δ} (P' ★ Q')%A.
 Proof. intros HP HQ. by rewrite HP, HQ. Qed.
-Lemma assert_sep_exist {A} Γ P (Q : A → assert K) :
-  (P ★ ∃ x, Q x)%A ≡{Γ} (∃ x, P ★ Q x)%A.
+Lemma assert_sep_exist {A} Γ δ P (Q : A → assert K) :
+  (P ★ ∃ x, Q x)%A ≡{Γ,δ} (∃ x, P ★ Q x)%A.
 Proof. solve eauto. Qed.
-Lemma assert_exist_sep {A} Γ (P : A → assert K) Q :
-  ((∃ x, P x) ★ Q)%A ≡{Γ} (∃ x, P x ★ Q)%A.
+Lemma assert_exist_sep {A} Γ δ (P : A → assert K) Q :
+  ((∃ x, P x) ★ Q)%A ≡{Γ,δ} (∃ x, P x ★ Q)%A.
 Proof. solve eauto. Qed.
-Lemma assert_wand_intro Γ P Q R : (P ★ Q)%A ⊆{Γ} R → P ⊆{Γ} (Q -★ R)%A.
+Lemma assert_wand_intro Γ δ P Q R : (P ★ Q)%A ⊆{Γ,δ} R → P ⊆{Γ,δ} (Q -★ R)%A.
 Proof.
-  intros HPQR Γ1 Δ1 ρ n m1 ???? HP Γ2 Δ2 n2 m2 ??????? HQ.
+  intros HPQR Γ1 Δ1 ρ δ1 n1 m1 ?????? HP Γ2 Δ2 δ2 n2 m2 ????????? HQ.
   apply HPQR; eauto using indexes_valid_weaken, cmap_union_valid_2.
   exists m1 m2; split_ands; eauto using assert_weaken, @sep_commutative.
 Qed.
-Lemma assert_wand_elim Γ P Q : ((P -★ Q) ★ P)%A ⊆{Γ} Q.
+Lemma assert_wand_elim Γ δ P Q : ((P -★ Q) ★ P)%A ⊆{Γ,δ} Q.
 Proof.
-  intros Γ1 Δ1 ρ n ????? (m1&m2&->&?&HQ&?).
+  intros Γ1 Δ1 ρ δ1 n ??????? (m1&m2&->&?&HQ&?).
   rewrite sep_commutative by auto; eapply HQ; eauto using
     cmap_valid_subseteq, @sep_union_subseteq_l, @sep_union_subseteq_r.
 Qed.
-Global Instance: LeftId (≡{Γ}) emp%A (-★)%A.
+Global Instance: LeftId (≡{Γ,δ}) emp%A (-★)%A.
 Proof.
   intros Γ P; split.
   * rewrite <-(right_id _ (★)%A); apply assert_wand_elim.
   * apply assert_wand_intro. by rewrite (right_id _ (★)%A).
 Qed.
 
-Lemma assert_Forall_holds_2 (Ps : list (assert K)) Γ Δ ρ ms n :
-  ⊥ ms → Forall2 (λ (P : assert K) m, assert_holds P Γ Δ ρ n m) Ps ms →
-  assert_holds (Π Ps)%A Γ Δ ρ n (⋃ ms).
+Lemma assert_Forall_holds_2 (Ps : list (assert K)) Γ Δ δ ρ ms n :
+  ⊥ ms → Forall2 (λ (P : assert K) m, assert_holds P Γ Δ δ ρ n m) Ps ms →
+  assert_holds (Π Ps)%A Γ Δ δ ρ n (⋃ ms).
 Proof. intros Hms HPs. revert Hms. induction HPs; solve eauto. Qed.
-Lemma assert_Forall_holds (Ps : list (assert K)) Γ Δ ρ n m :
-  assert_holds (Π Ps)%A Γ Δ ρ n m ↔ ∃ ms, m = ⋃ ms ∧ ⊥ ms ∧
-    Forall2 (λ (P : assert K) m, assert_holds P Γ Δ ρ n m) Ps ms.
+Lemma assert_Forall_holds (Ps : list (assert K)) Γ Δ δ ρ n m :
+  assert_holds (Π Ps)%A Γ Δ δ ρ n m ↔ ∃ ms, m = ⋃ ms ∧ ⊥ ms ∧
+    Forall2 (λ (P : assert K) m, assert_holds P Γ Δ δ ρ n m) Ps ms.
 Proof.
   split; [|naive_solver eauto using assert_Forall_holds_2].
   revert m. induction Ps as [|P Ps IH].
@@ -560,9 +569,9 @@ Proof.
   intros ? (m1&m2&->&?&?&?); destruct (IH m2) as (ms&->&?&?); trivial.
   exists (m1 :: ms); auto.
 Qed.
-Lemma assert_Forall_holds_vec {vn} (Ps : vec (assert K) vn) Γ Δ ρ n m :
-  assert_holds (Π Ps)%A Γ Δ ρ n m ↔ ∃ ms : vec _ vn, m = ⋃ ms ∧ ⊥ ms ∧
-    ∀ i, assert_holds (Ps !!! i) Γ Δ ρ n (ms !!! i).
+Lemma assert_Forall_holds_vec {vn} (Ps : vec (assert K) vn) Γ Δ δ ρ n m :
+  assert_holds (Π Ps)%A Γ Δ δ ρ n m ↔ ∃ ms : vec _ vn, m = ⋃ ms ∧ ⊥ ms ∧
+    ∀ i, assert_holds (Ps !!! i) Γ Δ δ ρ n (ms !!! i).
 Proof.
   rewrite assert_Forall_holds; split.
   * intros (ms&->&?&Hms). assert (vn = length ms); [|subst vn].
@@ -571,201 +580,204 @@ Proof.
     by rewrite <-(vec_to_list_of_list ms), Forall2_vlookup in Hms.
   * intros [ms ?]; exists ms; by rewrite Forall2_vlookup.
 Qed.
-Lemma assert_memext_l Γ P Q : MemExt P → (P ★ Q)%A ⊆{Γ} P.
+Lemma assert_memext_l Γ δ P Q : MemExt P → (P ★ Q)%A ⊆{Γ,δ} P.
 Proof.
   intros; transitivity (P ★ True)%A;
     auto using assert_sep_preserving, assert_True_intro.
 Qed.
-Lemma assert_memext_r Γ P Q : MemExt P → (Q ★ P)%A ⊆{Γ} P.
+Lemma assert_memext_r Γ δ P Q : MemExt P → (Q ★ P)%A ⊆{Γ,δ} P.
 Proof. rewrite (commutative (★)%A). apply assert_memext_l. Qed.
-Lemma assert_memext_l' Γ P Q R : MemExt R → P ⊆{Γ} R → (P ★ Q)%A ⊆{Γ} R.
+Lemma assert_memext_l' Γ δ P Q R : MemExt R → P ⊆{Γ,δ} R → (P ★ Q)%A ⊆{Γ,δ} R.
 Proof.
-  intros. rewrite <-(assert_memext_l _ R) by done.
+  intros. rewrite <-(assert_memext_l _ _ R) by done.
   eauto using assert_sep_preserving.
 Qed.
-Lemma assert_memext_r' Γ P Q R : MemExt R → Q ⊆{Γ} R → (P ★ Q)%A ⊆{Γ} R.
+Lemma assert_memext_r' Γ δ P Q R : MemExt R → Q ⊆{Γ,δ} R → (P ★ Q)%A ⊆{Γ,δ} R.
 Proof. rewrite (commutative (★)%A). apply assert_memext_l'. Qed.
 
 (* Evaluation and singleton connectives *)
 Global Instance assert_eval_memext e ν : MemExt (e ⇓ ν)%A.
 Proof.
-  intros Γ Γ' Δ ρ n m ?? Hm ? (m1&m2&->&?&(τlr&?&?)&?); exists τlr; split; auto.
+  intros Γ δ Γ' Δ δ' ρ n m ???? Hm ? (m1&m2&->&?&(τlr&?&?)&?).
+  exists τlr; split; auto.
   rewrite cmap_union_valid in Hm by auto; destruct Hm.
   eapply expr_eval_subseteq with _ m1 _; eauto using @sep_union_subseteq_l'.
 Qed.
-Lemma assert_int_typed_eval Γ P x τi :
-  int_typed x τi → P ⊆{Γ} (#intV{τi} x ⇓ inr (intV{τi} x))%A.
+Lemma assert_int_typed_eval Γ δ P x τi :
+  int_typed x τi → P ⊆{Γ,δ} (#intV{τi} x ⇓ inr (intV{τi} x))%A.
 Proof.
-  intros ? Γ' Δ ρ n m ?????.
+  intros ? Γ' Δ ρ δ' n m ??????.
   eexists (inr (intT τi)%T); split; auto using lockset_empty_valid.
 Qed.
-Lemma assert_eval_int_typed Γ e x τi :
-  (e ⇓ inr (intV{τi} x))%A ⊆{Γ} (⌜ int_typed x τi ⌝ ★ True)%A.
+Lemma assert_eval_int_typed Γ δ e x τi :
+  (e ⇓ inr (intV{τi} x))%A ⊆{Γ,δ} (⌜ int_typed x τi ⌝ ★ True)%A.
 Proof.
-  intros Γ' Δ ρ n m ???? (τlr&?&?).
+  intros Γ' Δ δ' ρ n m ?????? (τlr&?&?).
   assert ((Γ',Δ) ⊢ inr (intV{τi} x) : τlr) by eauto using expr_eval_typed.
   assert (sep_valid m) by eauto.
   typed_inversion_all; exists (∅ : mem K) m; eauto 9 using @sep_left_id, eq_sym.
 Qed.
-Lemma assert_eval_int_typed' Γ e x τi :
-  (e ⇓ inr (intV{τi} x))%A ⊆{Γ} (⌜ int_typed x τi ⌝ ★ e ⇓ inr (intV{τi} x))%A.
+Lemma assert_eval_int_typed' Γ δ e x τi :
+  (e ⇓ inr (intV{τi} x))%A ⊆{Γ,δ} (⌜ int_typed x τi ⌝ ★ e ⇓ inr (intV{τi} x))%A.
 Proof. eauto using assert_Prop_True, assert_eval_int_typed. Qed.
 Hint Extern 1 (unop_typed _ _ _) => constructor.
 Hint Extern 1 (base_unop_typed _ _ _) => constructor.
-Lemma assert_eval_int_unop Γ op e x τi :
+Lemma assert_eval_int_unop Γ δ op e x τi :
   int_unop_ok op x τi →
   (e ⇓ inr (intV{τi} x))%A
-  ⊆{Γ} (@{op} e ⇓ inr (intV{int_unop_type_of op τi} (int_unop op x τi)))%A.
+  ⊆{Γ,δ} (@{op} e ⇓ inr (intV{int_unop_type_of op τi} (int_unop op x τi)))%A.
 Proof.
-  intros ? Γ' Δ ρ n m ???? (τlr&?&?).
+  intros ? Γ' Δ δ' ρ n m ?????? (τlr&?&?).
   assert ((Γ',Δ) ⊢ inr (intV{τi} x) : τlr) by eauto using expr_eval_typed.
   typed_inversion_all;
     simplify_option_equality; eauto 20 using lockset_empty_valid.
 Qed.
-Lemma assert_eval_int_unop' Γ P op e x y τi σi :
-  P ⊆{Γ} (e ⇓ inr (intV{τi} x))%A →
+Lemma assert_eval_int_unop' Γ δ P op e x y τi σi :
+  P ⊆{Γ,δ} (e ⇓ inr (intV{τi} x))%A →
   int_unop_type_of op τi = σi → int_unop_ok op x τi → int_unop op x τi = y → 
-  P ⊆{Γ} (@{op} e ⇓ inr (intV{σi} y))%A.
+  P ⊆{Γ,δ} (@{op} e ⇓ inr (intV{σi} y))%A.
 Proof. intros; subst; rewrite <-assert_eval_int_unop by eauto; eauto. Qed.
 Hint Extern 1 (binop_typed _ _ _ _) => constructor.
 Hint Extern 1 (base_binop_typed _ _ _ _) => constructor.
-Lemma assert_eval_int_binop Γ op e1 e2 x1 x2 τi1 τi2 :
+Lemma assert_eval_int_binop Γ δ op e1 e2 x1 x2 τi1 τi2 :
   (int_binop_ok op x1 τi1 x2 τi2) →
-  (e1 ⇓ inr (intV{τi1} x1) ∧ e2 ⇓ inr (intV{τi2} x2))%A ⊆{Γ} (e1 @{op} e2 ⇓
-        inr (intV{int_binop_type_of op τi1 τi2} (int_binop op x1 τi1 x2 τi2)))%A.
+  (e1 ⇓ inr (intV{τi1} x1) ∧ e2 ⇓ inr (intV{τi2} x2))%A ⊆{Γ,δ} (e1 @{op} e2 ⇓
+       inr (intV{int_binop_type_of op τi1 τi2} (int_binop op x1 τi1 x2 τi2)))%A.
 Proof.
-  intros Hok Γ' Δ ρ n m ???? [(τlr1&?&?) (τlr2&?&?)].
+  intros Hok Γ' Δ δ' ρ n m ?????? [(τlr1&?&?) (τlr2&?&?)].
   assert ((Γ',Δ) ⊢ inr (intV{τi1} x1) : τlr1) by eauto using expr_eval_typed.
   assert ((Γ',Δ) ⊢ inr (intV{τi2} x2) : τlr2) by eauto using expr_eval_typed.
   typed_inversion_all.
   simplify_option_equality; eauto 20 using lockset_empty_valid.
 Qed.
-Lemma assert_eval_int_binop' Γ P op e1 e2 x1 x2 y τi1 τi2 σi :
-  P ⊆{Γ} (e1 ⇓ inr (intV{τi1} x1))%A → P ⊆{Γ} (e2 ⇓ inr (intV{τi2} x2))%A →
+Lemma assert_eval_int_binop' Γ δ P op e1 e2 x1 x2 y τi1 τi2 σi :
+  P ⊆{Γ,δ} (e1 ⇓ inr (intV{τi1} x1))%A → P ⊆{Γ,δ} (e2 ⇓ inr (intV{τi2} x2))%A →
   σi = int_binop_type_of op τi1 τi2 →
   int_binop_ok op x1 τi1 x2 τi2 → int_binop op x1 τi1 x2 τi2 = y →
-  P ⊆{Γ} (e1 @{op} e2 ⇓ inr (intV{σi} y))%A.
+  P ⊆{Γ,δ} (e1 @{op} e2 ⇓ inr (intV{σi} y))%A.
 Proof.
   intros; subst;
     rewrite <-assert_eval_int_binop by eauto; eauto using assert_and_intro.
 Qed.
-Lemma assert_eval_int_arithop' Γ P op e1 e2 x1 x2 y τi1 τi2 σi :
-  P ⊆{Γ} (e1 ⇓ inr (intV{τi1} x1))%A → P ⊆{Γ} (e2 ⇓ inr (intV{τi2} x2))%A →
+Lemma assert_eval_int_arithop' Γ δ P op e1 e2 x1 x2 y τi1 τi2 σi :
+  P ⊆{Γ,δ} (e1 ⇓ inr (intV{τi1} x1))%A → P ⊆{Γ,δ} (e2 ⇓ inr (intV{τi2} x2))%A →
   σi = int_promote τi1 ∪ int_promote τi2 →
   int_pre_arithop_ok op (int_pre_cast σi x1) (int_pre_cast σi x2) σi →
   int_pre_arithop op (int_pre_cast σi x1) (int_pre_cast σi x2) σi = y →
-  P ⊆{Γ} (e1 @{ArithOp op} e2 ⇓ inr (intV{σi} y))%A.
+  P ⊆{Γ,δ} (e1 @{ArithOp op} e2 ⇓ inr (intV{σi} y))%A.
 Proof.
   intros ?? -> ??.
-  rewrite assert_Prop_True by (rewrite <-(assert_eval_int_typed _ e1); auto).
+  rewrite assert_Prop_True by (rewrite <-(assert_eval_int_typed _ _ e1); auto).
   apply assert_Prop_intro_l; intros.
-  rewrite assert_Prop_True by (rewrite <-(assert_eval_int_typed _ e2); auto).
+  rewrite assert_Prop_True by (rewrite <-(assert_eval_int_typed _ _ e2); auto).
   apply assert_Prop_intro_l; intros; eapply assert_eval_int_binop'; eauto.
   * by apply int_arithop_ok_more.
   * unfold int_binop. by rewrite int_arithop_spec by auto.
 Qed.
 Hint Extern 1 (cast_typed _ _) => constructor.
 Hint Extern 1 (base_cast_typed _ _) => constructor.
-Lemma assert_eval_int_cast Γ e x τi σi :
+Lemma assert_eval_int_cast Γ δ e x τi σi :
   int_cast_ok σi x → 
   (e ⇓ inr (intV{τi} x))%A
-  ⊆{Γ} (cast{(intT σi)%T} e ⇓ inr (intV{σi} (int_cast σi x)))%A.
+  ⊆{Γ,δ} (cast{(intT σi)%T} e ⇓ inr (intV{σi} (int_cast σi x)))%A.
 Proof.
-  intros ? Γ' Δ ρ n m ???? (τlr&?&?).
+  intros ? Γ' Δ δ' ρ n m ?????? (τlr&?&?).
   assert ((Γ',Δ) ⊢ inr (intV{τi} x) : τlr) by eauto using expr_eval_typed.
   typed_inversion_all; simplify_option_equality.
   eauto 20 using lockset_empty_valid, TBase_valid, TInt_valid.
 Qed.
-Lemma assert_eval_int_cast' Γ P e x τi σi y :
-  P ⊆{Γ} (e ⇓ inr (intV{τi} x))%A →
+Lemma assert_eval_int_cast' Γ δ P e x τi σi y :
+  P ⊆{Γ,δ} (e ⇓ inr (intV{τi} x))%A →
   int_cast_ok σi x → int_cast σi x = y →
-  P ⊆{Γ} (cast{(intT σi)%T} e ⇓ inr (intV{σi} y))%A.
+  P ⊆{Γ,δ} (cast{(intT σi)%T} e ⇓ inr (intV{σi} y))%A.
 Proof. intros; subst; rewrite <-assert_eval_int_cast by eauto; eauto. Qed.
-Lemma assert_eval_int_cast_self' Γ P e x τi :
-  P ⊆{Γ} (e ⇓ inr (intV{τi} x))%A →
-  P ⊆{Γ} (cast{(intT τi)%T} e ⇓ inr (intV{τi} x))%A.
+Lemma assert_eval_int_cast_self' Γ δ P e x τi :
+  P ⊆{Γ,δ} (e ⇓ inr (intV{τi} x))%A →
+  P ⊆{Γ,δ} (cast{(intT τi)%T} e ⇓ inr (intV{τi} x))%A.
 Proof.
   intros HP. rewrite HP, assert_eval_int_typed'.
   eauto using assert_Prop_intro_l,
     assert_eval_int_cast', int_cast_ok_self, int_cast_self.
 Qed.
-Lemma assert_eval_singleton_l Γ a e μ γ τ :
-  (%a ↦{μ,γ} e : τ)%A ⊆{Γ} (%a ⇓ inl a)%A.
+Lemma assert_eval_singleton_l Γ δ a e μ γ τ :
+  (%a ↦{μ,γ} e : τ)%A ⊆{Γ,δ} (%a ⇓ inl a)%A.
 Proof.
-  intros Γ' Δ ρ n m ???? (a'&v&?&?&?&?&?);
+  intros Γ' Δ δ' ρ n m ?????? (a'&v&?&?&?&?&?);
     eexists (inl τ); simplify_option_equality; eauto.
 Qed.
-Lemma assert_eval_singleton_r Γ e v μ γ τ :
-  (e ↦{μ,γ} #v : τ)%A ⊆{Γ} (#v ⇓ inr v)%A.
+Lemma assert_eval_singleton_r Γ δ e v μ γ τ :
+  (e ↦{μ,γ} #v : τ)%A ⊆{Γ,δ} (#v ⇓ inr v)%A.
 Proof.
-  intros Γ' Δ ρ n m ???? (a&v'&?&?&?&?&?);
+  intros Γ' Δ δ' ρ n m ?????? (a&v'&?&?&?&?&?);
     eexists (inr τ); simplify_option_equality; eauto.
 Qed.
-Lemma assert_singleton_l Γ e1 e2 μ γ τ :
-  (e1 ↦{μ,γ} e2 : τ)%A ≡{Γ} (∃ a, (e1 ⇓ inl a ∧ emp) ★ %a ↦{μ,γ} e2 : τ)%A.
+Lemma assert_singleton_l Γ δ e1 e2 μ γ τ :
+  (e1 ↦{μ,γ} e2 : τ)%A ≡{Γ,δ} (∃ a, (e1 ⇓ inl a ∧ emp) ★ %a ↦{μ,γ} e2 : τ)%A.
 Proof.
   split.
-  * intros Γ' Δ ρ n m ???? (a&v&?&?&?&?&?); exists a.
+  * intros Γ' Δ δ' ρ n m ?????? (a&v&?&?&?&?&?); exists a.
     assert (sep_valid m) by eauto using cmap_valid_sep_valid.
     eexists ∅, m; split_ands; simplify_option_equality; eauto 20 using
       @sep_left_id, eq_sym, lockset_empty_valid, mem_singleton_typed_addr_typed.
-  * intros Γ' Δ ρ n m_ ?? Hm ? (?&?&m&->&?&((τlr&?&?)&_&->)&(a&v&?&?&?&?&?));
-      simplify_option_equality.
+  * intros Γ' Δ δ' ρ n m_ ???? Hm ?
+      (?&?&m&->&?&((τlr&?&?)&_&->)&(a&v&?&?&?&?&?)); simplify_option_equality.
     exists a v; rewrite sep_left_id in Hm |- * by auto; split_ands; auto.
     cut (τlr = inl τ); [intros ->; auto|typed_inversion_all].
     apply (typed_unique (Γ',Δ) (inl a));
       eauto using expr_eval_typed, cmap_empty_valid, cmap_valid_memenv_valid.
 Qed.
-Lemma assert_singleton_l_2 Γ e1 e2 μ γ a τ :
-  ((e1 ⇓ inl a ∧ emp) ★ %a ↦{μ,γ} e2 : τ)%A ⊆{Γ} (e1 ↦{μ,γ} e2 : τ)%A.
-Proof. rewrite (assert_singleton_l _ e1); solve eauto. Qed.
-Lemma assert_singleton_l_ Γ e μ γ τ :
-  (e ↦{μ,γ} - : τ)%A ≡{Γ} (∃ a, (e ⇓ inl a ∧ emp) ★ %a ↦{μ,γ} - : τ)%A.
+Lemma assert_singleton_l_2 Γ δ e1 e2 μ γ a τ :
+  ((e1 ⇓ inl a ∧ emp) ★ %a ↦{μ,γ} e2 : τ)%A ⊆{Γ,δ} (e1 ↦{μ,γ} e2 : τ)%A.
+Proof. rewrite (assert_singleton_l _ _ e1); solve eauto. Qed.
+Lemma assert_singleton_l_ Γ δ e μ γ τ :
+  (e ↦{μ,γ} - : τ)%A ≡{Γ,δ} (∃ a, (e ⇓ inl a ∧ emp) ★ %a ↦{μ,γ} - : τ)%A.
 Proof.
-  setoid_rewrite (assert_singleton_l Γ e); setoid_rewrite (assert_sep_exist Γ).
-  by rewrite assert_exist_exist.
+  setoid_rewrite (assert_singleton_l Γ δ e).
+  by setoid_rewrite (assert_sep_exist Γ δ); rewrite assert_exist_exist.
 Qed.
-Lemma assert_singleton_l_2_ Γ e μ γ a τ :
-  ((e ⇓ inl a ∧ emp) ★ %a ↦{μ,γ} - : τ)%A ⊆{Γ} (e ↦{μ,γ} - : τ)%A.
-Proof. rewrite (assert_singleton_l_ _ e); solve eauto. Qed.
-Lemma assert_singleton_int_typed Γ e μ γ z τi :
-  (e ↦{μ,γ} #intV{τi} z : intT τi)%A ⊆{Γ} (⌜ int_typed z τi ⌝ ★ True)%A.
+Lemma assert_singleton_l_2_ Γ δ e μ γ a τ :
+  ((e ⇓ inl a ∧ emp) ★ %a ↦{μ,γ} - : τ)%A ⊆{Γ,δ} (e ↦{μ,γ} - : τ)%A.
+Proof. rewrite (assert_singleton_l_ _ _ e); solve eauto. Qed.
+Lemma assert_singleton_int_typed Γ δ e μ γ z τi :
+  (e ↦{μ,γ} #intV{τi} z : intT τi)%A ⊆{Γ,δ} (⌜ int_typed z τi ⌝ ★ True)%A.
 Proof. rewrite assert_eval_singleton_r; apply assert_eval_int_typed. Qed.
-Lemma assert_singleton_int_typed' Γ e μ γ z τi :
+Lemma assert_singleton_int_typed' Γ δ e μ γ z τi :
   (e ↦{μ,γ} #intV{τi} z : intT τi)%A
-  ⊆{Γ} (⌜ int_typed z τi ⌝ ★ (e ↦{μ,γ} #intV{τi} z : intT τi))%A.
+  ⊆{Γ,δ} (⌜ int_typed z τi ⌝ ★ (e ↦{μ,γ} #intV{τi} z : intT τi))%A.
 Proof. by apply assert_Prop_True, assert_singleton_int_typed. Qed.
-Lemma assert_expr_lift Γ e ν : vars e = ∅ → (e↑ ⇓ ν)%A ≡{Γ} (e ⇓ ν)%A.
+Lemma assert_expr_lift Γ δ e ν : vars e = ∅ → (e↑ ⇓ ν)%A ≡{Γ,δ} (e ⇓ ν)%A.
 Proof.
-  split; intros Γ' Δ ρ n m ???? (τlr&?&?); exists τlr; split.
+  split; intros Γ' Δ δ' ρ n m ?????? (τlr&?&?); exists τlr; split.
   * by apply expr_typed_var_free with (tail (ρ.*2)), expr_typed_lift.
   * erewrite expr_eval_var_free, <-expr_eval_lift; eauto.
   * eapply expr_typed_lift, expr_typed_var_free; eauto.
   * erewrite expr_eval_lift, <-expr_eval_var_free by done; eauto.
 Qed.
-Lemma assert_singleton_lift_l Γ e1 e2 μ γ τ :
-  vars e1 = ∅ → (e1↑ ↦{μ,γ} e2 : τ)%A ≡{Γ} (e1 ↦{μ,γ} e2 : τ)%A.
+Lemma assert_singleton_lift_l Γ δ e1 e2 μ γ τ :
+  vars e1 = ∅ → (e1↑ ↦{μ,γ} e2 : τ)%A ≡{Γ,δ} (e1 ↦{μ,γ} e2 : τ)%A.
 Proof.
-  split; intros Γ' Δ ρ n m ???? (a&v&?&?&?&?&?); exists a v; split_ands; auto.
+  split; intros Γ' Δ δ' ρ n m ?????? (a&v&?&?&?&?&?);
+    exists a v; split_ands; auto.
   * by apply expr_typed_var_free with (tail (ρ.*2)), expr_typed_lift.
   * erewrite expr_eval_var_free, <-expr_eval_lift; eauto.
   * eapply expr_typed_lift, expr_typed_var_free; eauto.
   * erewrite expr_eval_lift, <-expr_eval_var_free by done; eauto.
 Qed.
-Lemma assert_singleton_lift_r Γ e1 e2 μ γ τ :
-  vars e2 = ∅ → (e1 ↦{μ,γ} (e2↑) : τ)%A ≡{Γ} (e1 ↦{μ,γ} e2 : τ)%A.
+Lemma assert_singleton_lift_r Γ δ e1 e2 μ γ τ :
+  vars e2 = ∅ → (e1 ↦{μ,γ} (e2↑) : τ)%A ≡{Γ,δ} (e1 ↦{μ,γ} e2 : τ)%A.
 Proof.
-  split; intros Γ' Δ ρ n m ???? (a&v&?&?&?&?&?); exists a v; split_ands; auto.
+  split; intros Γ' Δ δ' ρ n m ?????? (a&v&?&?&?&?&?);
+    exists a v; split_ands; auto.
   * by apply expr_typed_var_free with (tail (ρ.*2)), expr_typed_lift.
   * erewrite expr_eval_var_free, <-expr_eval_lift; eauto.
   * eapply expr_typed_lift, expr_typed_var_free; eauto.
   * erewrite expr_eval_lift, <-expr_eval_var_free by done; eauto.
 Qed.
-Lemma assert_singleton_eval Γ e v μ γ τ :
-  Some Readable ⊆ perm_kind γ → (e ↦{μ,γ} #v : τ)%A ⊆{Γ} (load e ⇓ inr v)%A.
+Lemma assert_singleton_eval Γ δ e v μ γ τ :
+  Some Readable ⊆ perm_kind γ → (e ↦{μ,γ} #v : τ)%A ⊆{Γ,δ} (load e ⇓ inr v)%A.
 Proof.
-  intros ? Γ1 Δ1 ρ n ????? (a&v'&?&?&?&?&?); simplify_option_equality.
-  assert (✓{Γ1} Δ1) by eauto using cmap_valid_memenv_valid.
+  intros ? Γ1 Δ δ' ρ n ??????? (a&v'&?&?&?&?&?); simplify_option_equality.
+  assert (✓{Γ1} Δ) by eauto using cmap_valid_memenv_valid.
   eexists (inr τ); split_ands; auto.
   erewrite (expr_eval_weaken _ _ _ _ _ ∅) by eauto using cmap_empty_valid,
     cmap_subseteq_index_alive, mem_lookup_subseteq, mem_forced_subseteq,
@@ -773,24 +785,25 @@ Proof.
   by erewrite option_guard_True, mem_lookup_singleton
     by eauto using mem_singleton_forced.
 Qed.
-Lemma assert_singleton_union_lr Γ e1 e2 μ γ1 γ2 τ :
+Lemma assert_singleton_union_lr Γ δ e1 e2 μ γ1 γ2 τ :
   ⊥[γ1;γ2] → ¬sep_unmapped γ1 → ¬sep_unmapped γ2 →
-  (e1 ↦{μ,γ1 ∪ γ2} e2 : τ)%A ≡{Γ} (e1 ↦{μ,γ1} e2 : τ ★ e1 ↦{μ,γ2} e2 : τ)%A.
+  (e1 ↦{μ,γ1 ∪ γ2} e2 : τ)%A ≡{Γ,δ} (e1 ↦{μ,γ1} e2 : τ ★ e1 ↦{μ,γ2} e2 : τ)%A.
 Proof.
   intros; split.
-  * intros Γ1 Δ1 ρ n ????? (a&v&?&?&?&?&?).
-    destruct (mem_singleton_union_rev Γ1 Δ1 m a μ γ1 γ2 v τ)
+  * intros Γ1 Δ δ' ρ n ??????? (a&v&?&?&?&?&?).
+    destruct (mem_singleton_union_rev Γ1 Δ m a μ γ1 γ2 v τ)
       as (m1&m2&->&?&?&?); auto.
     exists m1 m2; split_ands; solve ltac:eauto.
-  * intros Γ1 Δ1 ρ n ????? (?&?&->&?&(a1&v1&?&?&?&?&?)&(a2&v2&?&?&?&?&?));
+  * intros Γ1 Δ δ' ρ n ??????? (?&?&->&?&(a1&v1&?&?&?&?&?)&(a2&v2&?&?&?&?&?));
       simplify_equality'; exists a1 v1; eauto 10 using mem_singleton_union.
 Qed.
-Lemma assert_singleton_union_l Γ e1 e2 μ γ1 γ2 τ :
+Lemma assert_singleton_union_l Γ δ e1 e2 μ γ1 γ2 τ :
   ⊥[γ1;γ2] → ¬sep_unmapped γ1 → γ2 ≠ ∅ →
-  (e1 ↦{μ,γ1 ∪ γ2} e2 : τ)%A ≡{Γ} (e1 ↦{μ,γ1} e2 : τ ★ e1 ↦{μ,γ2} - : τ)%A.
+  (e1 ↦{μ,γ1 ∪ γ2} e2 : τ)%A ≡{Γ,δ} (e1 ↦{μ,γ1} e2 : τ ★ e1 ↦{μ,γ2} - : τ)%A.
 Proof.
   intros; split.
-  * intros Γ1 Δ1 ρ n ????? (a&v&?&?&?&?&?); destruct (decide (sep_unmapped γ2)).
+  * intros Γ1 Δ1 δ1 ρ n ??????? (a&v&?&?&?&?&?).
+    destruct (decide (sep_unmapped γ2)).
     + destruct (mem_singleton_union_rev_unmapped Γ1 Δ1 m a μ γ1 γ2 v τ)
         as (m1&m2&->&?&?&?); auto using @sep_unmapped_empty_alt.
       assert ((Γ1,Δ1) ⊢ val_new Γ1 τ : τ).
@@ -802,57 +815,59 @@ Proof.
         as (m1&m2&->&?&?&?); auto.
       exists m1 m2; solve ltac:(eauto using expr_eval_typed,
         lockset_empty_valid, cmap_empty_valid, cmap_valid_memenv_valid).
-  * intros Γ1 Δ1 ρ n ????? (?&?&->&?&(a1&v1&?&?&?&?&?)&(?&a2&v2&?&?&?&?&?));
+  * intros Γ1 Δ1 δ1 ρ n ???????
+      (?&?&->&?&(a1&v1&?&?&?&?&?)&(?&a2&v2&?&?&?&?&?));
       simplify_option_equality; exists a1 v1; split_ands; auto.
     by eapply (mem_singleton_union _ _ _ _ _ _ _ _ v1 v2); eauto.
 Qed.
-Lemma assert_singleton_union_r Γ e1 e2 μ γ1 γ2 τ :
+Lemma assert_singleton_union_r Γ δ e1 e2 μ γ1 γ2 τ :
   ⊥[γ1;γ2] → γ1 ≠ ∅ → ¬sep_unmapped γ2 →
-  (e1 ↦{μ,γ1 ∪ γ2} e2 : τ)%A ≡{Γ} (e1 ↦{μ,γ1} - : τ ★ e1 ↦{μ,γ2} e2 : τ)%A.
+  (e1 ↦{μ,γ1 ∪ γ2} e2 : τ)%A ≡{Γ,δ} (e1 ↦{μ,γ1} - : τ ★ e1 ↦{μ,γ2} e2 : τ)%A.
 Proof.
   intros. rewrite (commutative (★)%A), sep_commutative by auto.
   by rewrite assert_singleton_union_l by auto.
 Qed.
-Lemma assert_singleton_union Γ e1 μ γ1 γ2 τ :
+Lemma assert_singleton_union Γ δ e1 μ γ1 γ2 τ :
   ⊥[γ1;γ2] → γ1 ≠ ∅ → γ2 ≠ ∅ →
-  (e1 ↦{μ,γ1 ∪ γ2} - : τ)%A ≡{Γ} (e1 ↦{μ,γ1} - : τ ★ e1 ↦{μ,γ2} - : τ)%A.
+  (e1 ↦{μ,γ1 ∪ γ2} - : τ)%A ≡{Γ,δ} (e1 ↦{μ,γ1} - : τ ★ e1 ↦{μ,γ2} - : τ)%A.
 Proof.
   intros; split.
-  * intros Γ1 Δ1 ρ n ????? (?&a&v&?&?&?&?&?); simplify_option_equality;
+  * intros Γ1 Δ δ1 ρ n ??????? (?&a&v&?&?&?&?&?); simplify_option_equality;
       typed_inversion_all; destruct (decide (sep_unmapped γ2)).
-    { destruct (mem_singleton_union_rev_unmapped Γ1 Δ1 m a μ γ1 γ2 v τ)
+    { destruct (mem_singleton_union_rev_unmapped Γ1 Δ m a μ γ1 γ2 v τ)
         as (m1&m2&->&?&?&?); auto using @sep_unmapped_empty_alt.
-      assert ((Γ1,Δ1) ⊢ val_new Γ1 τ : τ).
+      assert ((Γ1,Δ) ⊢ val_new Γ1 τ : τ).
       { eauto using val_new_typed,
           mem_singleton_typed_addr_typed, addr_typed_type_valid. }
       exists m1 m2; split_ands; eauto 10 using lockset_empty_valid. }
     destruct (decide (sep_unmapped γ1)).
-    { destruct (mem_singleton_union_rev_unmapped Γ1 Δ1 m a μ γ2 γ1 v τ)
+    { destruct (mem_singleton_union_rev_unmapped Γ1 Δ m a μ γ2 γ1 v τ)
         as (m1&m2&->&?&?&?); auto using @sep_unmapped_empty_alt.
       { by rewrite sep_commutative by auto. }
-      assert ((Γ1,Δ1) ⊢ val_new Γ1 τ : τ).
+      assert ((Γ1,Δ) ⊢ val_new Γ1 τ : τ).
       { eauto using val_new_typed,
           mem_singleton_typed_addr_typed, addr_typed_type_valid. }
       exists m2 m1; eauto 30 using @sep_commutative. }
-    destruct (mem_singleton_union_rev Γ1 Δ1 m a μ γ1 γ2 v τ)
+    destruct (mem_singleton_union_rev Γ1 Δ m a μ γ1 γ2 v τ)
       as (m1&m2&->&?&?&?); eauto 40.
-  * intros Γ1 Δ1 ρ n ????? (?&?&->&?&(?&a1&v1&?&?&?&?&?)&(?&a2&v2&?&?&?&?&?));
+  * intros Γ1 Δ δ1 ρ n ???????
+      (?&?&->&?&(?&a1&v1&?&?&?&?&?)&(?&a2&v2&?&?&?&?&?));
       simplify_option_equality; destruct (decide (sep_unmapped γ1)).
     + eexists v2, a1, v2; split_ands; eauto.
       by eapply (mem_singleton_union _ _ _ _ _ _ _ _ v1 v2); eauto.
     + eexists v1, a1, v1; split_ands; eauto.
       by eapply (mem_singleton_union _ _ _ _ _ _ _ _ v1 v2); eauto.
 Qed.
-Lemma assert_singleton_array Γ e μ γ vs τ n :
+Lemma assert_singleton_array Γ δ e μ γ vs τ n :
   length vs = n → n ≠ 0 →
   (e ↦{μ,γ} #(VArray τ vs) : (τ.[n]))%A
-  ≡{Γ} (Π imap (λ i v, (e %> RArray i τ n) ↦{μ,γ} #v : τ) vs)%A.
+  ≡{Γ,δ} (Π imap (λ i v, (e %> RArray i τ n) ↦{μ,γ} #v : τ) vs)%A.
 Proof.
   intros Hn Hn'. split.
-  * intros Γ1 Δ1 ρ n' ??? Hm ? (a&v&?&?&_&Hvs&w&->&->&Hw&Hw'&Ha&_&?&?).
+  * intros Γ1 Δ δ1 ρ n' ????? Hm ? (a&v&?&?&_&Hvs&w&->&->&Hw&Hw'&Ha&_&?&?).
     apply cmap_valid_memenv_valid in Hm; clear Hn Hn'.
     assert (∃ ws, w = MArray τ ws ∧ length ws = n ∧
-      vs = to_val Γ1 <$> ws ∧ (Γ1,Δ1) ⊢* ws : τ) as (ws&->&Hn&->&Hws).
+      vs = to_val Γ1 <$> ws ∧ (Γ1,Δ) ⊢* ws : τ) as (ws&->&Hn&->&Hws).
     { destruct w; simplify_option_equality; typed_inversion_all; eauto. }
     assert (Forall (not ∘ Forall (∅ =) ∘ ctree_flatten) ws) as Hemp.
     { clear Hn Hw Hvs.
@@ -867,9 +882,10 @@ Proof.
     + by simplify_option_equality.
     + typed_constructor; eauto using to_val_typed, lockset_empty_valid.
     + exists w; eauto 12 using addr_elt_is_obj, addr_elt_strict, addr_elt_typed.
-  * intros Γ1 Δ1 ρ n' m _ ? Hm ?; rewrite assert_Forall_holds; intros (ms&->&_&Hms).
+  * intros Γ1 Δ δ1 ρ n' m _ ??? Hm ?.
+    rewrite assert_Forall_holds; intros (ms&->&_&Hms).
     apply cmap_valid_memenv_valid in Hm.
-    assert (∃ a, (Γ1,Δ1,ρ.*2) ⊢ e : inl (τ.[n])%T ∧
+    assert (∃ a, (Γ1,Δ,ρ.*2) ⊢ e : inl (τ.[n])%T ∧
       ⟦ e ⟧ Γ1 ρ ∅ = Some (inl a) ∧ addr_strict Γ1 a ∧ γ ≠ ∅) as (a&He&?&?&?).
     { unfold imap in *; destruct vs; decompose_Forall_hyps.
       match goal with
@@ -877,7 +893,7 @@ Proof.
       end; simplify_option_equality; typed_inversion_all; eauto. }
     assert (∃ ws,
       ms = imap (λ i, cmap_singleton Γ1 (addr_elt Γ1 (RArray i τ n) a) μ) ws ∧
-      vs = to_val Γ1 <$> ws ∧ (Γ1,Δ1) ⊢* ws : τ ∧
+      vs = to_val Γ1 <$> ws ∧ (Γ1,Δ) ⊢* ws : τ ∧
       Forall (λ γb, tagged_perm γb = γ) (ws ≫= ctree_flatten))
       as (ws&->&->&Hws&Hws').
     { cut (0 + length vs ≤ n); [|lia]; unfold imap in *.
@@ -893,9 +909,9 @@ Proof.
     { clear Hn Hms.
       induction Hws as [|w ws]; constructor; decompose_Forall_hyps; eauto.
       eapply ctree_Forall_not, Forall_impl; naive_solver. }
-    assert ((Γ1,Δ1) ⊢* to_val Γ1 <$> ws : τ).
+    assert ((Γ1,Δ) ⊢* to_val Γ1 <$> ws : τ).
     { eapply Forall_fmap; eauto using Forall_impl, to_val_typed. }
-    assert ((Γ1,Δ1) ⊢ a : TType (τ.[n])) by eauto 10
+    assert ((Γ1,Δ) ⊢ a : TType (τ.[n])) by eauto 10
       using lval_typed_inv, expr_eval_typed, cmap_empty_valid.
     exists a (VArray τ (to_val Γ1 <$> ws));
       split_ands; eauto using lockset_empty_valid.
@@ -906,41 +922,43 @@ Proof.
 Qed.
 
 (* Lifting De Bruijn indexes *)
-Global Instance: Proper ((⊆{Γ}) ==> (⊆{Γ})) assert_lift.
+Global Instance: Proper ((⊆{Γ,δ}) ==> (⊆{Γ,δ})) assert_lift.
 Proof. solve ltac:(eauto using Forall_tail). Qed.
-Global Instance: Proper ((≡{Γ}) ==> (≡{Γ})) assert_lift.
+Global Instance: Proper ((≡{Γ,δ}) ==> (≡{Γ,δ})) assert_lift.
 Proof. solve ltac:(eauto using Forall_tail). Qed.
 
-Lemma assert_lift_impl Γ P Q : ((P → Q)↑)%A ≡{Γ} (P↑ → Q↑)%A.
+Lemma assert_lift_impl Γ δ P Q : ((P → Q)↑)%A ≡{Γ,δ} (P↑ → Q↑)%A.
 Proof. solve eauto. Qed.
-Lemma assert_lift_and Γ P Q : ((P ∧ Q)↑)%A ≡{Γ} (P↑ ∧ Q↑)%A.
+Lemma assert_lift_and Γ δ P Q : ((P ∧ Q)↑)%A ≡{Γ,δ} (P↑ ∧ Q↑)%A.
 Proof. solve eauto. Qed.
-Lemma assert_lift_or Γ P Q : ((P ∨ Q)↑)%A ≡{Γ} (P↑ ∨ Q↑)%A.
+Lemma assert_lift_or Γ δ P Q : ((P ∨ Q)↑)%A ≡{Γ,δ} (P↑ ∨ Q↑)%A.
 Proof. solve eauto. Qed.
-Lemma assert_lift_not Γ P : ((¬P)↑)%A ≡{Γ} (¬P↑)%A.
+Lemma assert_lift_not Γ δ P : ((¬P)↑)%A ≡{Γ,δ} (¬P↑)%A.
 Proof. solve eauto. Qed.
-Lemma assert_lift_forall Γ {A} (P : A → assert K) :
-  ((∀ x, P x)↑)%A ≡{Γ} (∀ x, P x↑)%A.
+Lemma assert_lift_forall Γ δ {A} (P : A → assert K) :
+  ((∀ x, P x)↑)%A ≡{Γ,δ} (∀ x, P x↑)%A.
 Proof. solve eauto. Qed.
-Lemma assert_lift_exists Γ {A} (P : A → assert K) :
-  ((∃ x, P x)↑)%A ≡{Γ} (∃ x, P x↑)%A.
+Lemma assert_lift_exists Γ δ {A} (P : A → assert K) :
+  ((∃ x, P x)↑)%A ≡{Γ,δ} (∃ x, P x↑)%A.
 Proof. solve eauto. Qed.
-Lemma assert_lift_sep Γ P Q : ((P ★ Q)↑)%A ≡{Γ} (P↑ ★ Q↑)%A.
+Lemma assert_lift_sep Γ δ P Q : ((P ★ Q)↑)%A ≡{Γ,δ} (P↑ ★ Q↑)%A.
 Proof. solve eauto. Qed.
-Lemma assert_lift_wand Γ P Q : ((P -★ Q)↑)%A ≡{Γ} (P↑ -★ Q↑)%A.
+Lemma assert_lift_wand Γ δ P Q : ((P -★ Q)↑)%A ≡{Γ,δ} (P↑ -★ Q↑)%A.
 Proof. solve eauto. Qed.
-Lemma assert_lift_expr Γ e v : ((e ⇓ v)↑)%A ≡{Γ} (e↑ ⇓ v)%A.
+Lemma assert_lift_expr Γ δ e v : ((e ⇓ v)↑)%A ≡{Γ,δ} (e↑ ⇓ v)%A.
 Proof.
   split.
-  * intros Γ' Δ ρ n m ???? (τlr&?&?); exists τlr.
+  * intros Γ' Δ δ' ρ n m ?????? (τlr&?&?); exists τlr.
     by rewrite expr_eval_lift, expr_typed_lift, <-fmap_tail.
-  * intros Γ' Δ ρ n m ???? (τlr&?&?); exists τlr.
+  * intros Γ' Δ δ' ρ n m ?????? (τlr&?&?); exists τlr.
     by rewrite fmap_tail, <-expr_eval_lift, <-expr_typed_lift.
 Qed.
-Lemma assert_lift_expr_ Γ e : ((e ⇓ -)↑)%A ≡{Γ} (e↑ ⇓ -)%A.
-Proof. by rewrite assert_lift_exists; setoid_rewrite (assert_lift_expr Γ). Qed.
-Lemma assert_lift_singleton Γ e1 e2 μ γ τ :
-  ((e1 ↦{μ,γ} e2 : τ)↑)%A ≡{Γ} ((e1↑) ↦{μ,γ} (e2↑) : τ)%A.
+Lemma assert_lift_expr_ Γ δ e : ((e ⇓ -)↑)%A ≡{Γ,δ} (e↑ ⇓ -)%A.
+Proof.
+  by rewrite assert_lift_exists; setoid_rewrite (assert_lift_expr Γ δ).
+Qed.
+Lemma assert_lift_singleton Γ δ e1 e2 μ γ τ :
+  ((e1 ↦{μ,γ} e2 : τ)↑)%A ≡{Γ,δ} ((e1↑) ↦{μ,γ} (e2↑) : τ)%A.
 Proof.
   split; repeat intro.
   * do 2 red. by setoid_rewrite expr_eval_lift;
@@ -948,14 +966,14 @@ Proof.
   * do 4 red. by rewrite fmap_tail; setoid_rewrite <-expr_eval_lift;
       setoid_rewrite <-expr_typed_lift.
 Qed.
-Lemma assert_lift_singleton_ Γ e1 μ γ τ :
-  ((e1 ↦{μ,γ} - : τ)↑)%A ≡{Γ} ((e1↑) ↦{μ,γ} - : τ)%A.
+Lemma assert_lift_singleton_ Γ δ e1 μ γ τ :
+  ((e1 ↦{μ,γ} - : τ)↑)%A ≡{Γ,δ} ((e1↑) ↦{μ,γ} - : τ)%A.
 Proof.
-  by rewrite assert_lift_exists; setoid_rewrite (assert_lift_singleton Γ).
+  by rewrite assert_lift_exists; setoid_rewrite (assert_lift_singleton Γ δ).
 Qed.
 
 Global Instance assert_lift_stack_indep: StackIndep P → StackIndep (P↑).
-Proof. intros P ? Γ. by rewrite !stack_indep. Qed.
+Proof. intros P ? Γ δ; by rewrite !stack_indep. Qed.
 Global Instance assert_True_stack_indep : StackIndep True.
 Proof. solve eauto. Qed.
 Global Instance assert_False_stack_indep : StackIndep False.
@@ -964,7 +982,7 @@ Global Instance assert_Prop_stack_indep P : StackIndep (⌜ P ⌝).
 Proof. solve eauto. Qed.
 Global Instance assert_impl_stack_indep :
   StackIndep P → StackIndep Q → StackIndep (P → Q).
-Proof. by intros P Q ?? Γ; rewrite assert_lift_impl, !stack_indep. Qed.
+Proof. by intros P Q ?? Γ δ; rewrite assert_lift_impl, !stack_indep. Qed.
 Global Instance assert_and_stack_indep :
   StackIndep P → StackIndep Q → StackIndep (P ∧ Q).
 Proof. solve eauto. Qed.
@@ -979,100 +997,100 @@ Global Instance assert_exist_stack_indep A :
 Proof. solve eauto. Qed.
 Global Instance assert_sep_stack_indep :
   StackIndep P → StackIndep Q → StackIndep (P ★ Q).
-Proof. by intros P Q HP HQ Γ; rewrite assert_lift_sep, !stack_indep. Qed.
+Proof. by intros P Q HP HQ Γ δ; rewrite assert_lift_sep, !stack_indep. Qed.
 Global Instance assert_wand_stack_indep :
   StackIndep P → StackIndep Q → StackIndep (P -★ Q).
-Proof. by intros P Q ?? Γ; rewrite assert_lift_wand, !stack_indep. Qed.
+Proof. by intros P Q ?? Γ δ; rewrite assert_lift_wand, !stack_indep. Qed.
 Global Instance assert_expr_stack_indep e v : vars e = ∅ → StackIndep (e ⇓ v).
-Proof. intros ? Γ. by rewrite assert_lift_expr, assert_expr_lift. Qed.
+Proof. intros ? Γ δ. by rewrite assert_lift_expr, assert_expr_lift. Qed.
 Global Instance assert_singleton_stack_indep e1 e2 μ γ τ :
   vars e1 = ∅ → vars e2 = ∅ → StackIndep (e1 ↦{μ,γ} e2 : τ).
 Proof.
-  by intros ?? Γ; rewrite assert_lift_singleton,
+  by intros ?? Γ δ; rewrite assert_lift_singleton,
     assert_singleton_lift_l, assert_singleton_lift_r by done.
 Qed.
-Lemma stack_indep_spec P Γ Δ ρ1 ρ2 n m :
-  StackIndep P → ✓ Γ → ✓{Γ,Δ} m → ✓{Δ}* ρ1 → ✓{Δ}* ρ2 →
-  assert_holds P Γ Δ ρ1 n m → assert_holds P Γ Δ ρ2 n m.
+Lemma stack_indep_spec P Γ Δ δ ρ1 ρ2 n m :
+  StackIndep P → ✓ Γ → ✓{Γ,Δ} δ → ✓{Γ,Δ} m → ✓{Δ}* ρ1 → ✓{Δ}* ρ2 →
+  assert_holds P Γ Δ δ ρ1 n m → assert_holds P Γ Δ δ ρ2 n m.
 Proof.
-  intros HP ?? Hρ1 Hρ2 ?; assert (assert_holds P Γ Δ [] n m).
+  intros HP ??? Hρ1 Hρ2 ?; assert (assert_holds P Γ Δ δ [] n m).
   * induction Hρ1 as [|[o τ] ρ ?? IH]; auto.
-    eapply IH, (proj2 (HP _) Γ Δ (_ :: _)); eauto.
+    eapply IH, (proj2 (HP _ _) Γ Δ δ (_ :: _)); simpl; eauto.
   * induction Hρ2 as [|[o τ] ρ ?? IH]; auto.
-    eapply (proj1 (HP _)), IH; eauto.
+    eapply (proj1 (HP _ _)), IH; simpl; eauto.
 Qed.
 
 (* Unlocking *)
-Lemma assert_unlock_spec P Γ Δ ρ n m :
-  assert_holds (P ◊) Γ Δ ρ n m = assert_holds P Γ Δ ρ n (mem_unlock_all m).
+Lemma assert_unlock_spec P Γ Δ δ ρ n m :
+  assert_holds (P ◊) Γ Δ δ ρ n m = assert_holds P Γ Δ δ ρ n (mem_unlock_all m).
 Proof. done. Qed.
-Global Instance: Proper ((⊆{Γ}) ==> (⊆{Γ})) assert_unlock.
+Global Instance: Proper ((⊆{Γ,δ}) ==> (⊆{Γ,δ})) assert_unlock.
 Proof. solve ltac:(eauto using mem_unlock_all_valid). Qed.
-Global Instance: Proper ((≡{Γ}) ==> (≡{Γ})) assert_unlock.
+Global Instance: Proper ((≡{Γ,δ}) ==> (≡{Γ,δ})) assert_unlock.
 Proof. solve ltac:(eauto using mem_unlock_all_valid). Qed.
 
-Lemma assert_unlock_unlock Γ P : (P ◊ ◊)%A ≡{Γ} (P ◊)%A.
+Lemma assert_unlock_unlock Γ δ P : (P ◊ ◊)%A ≡{Γ,δ} (P ◊)%A.
 Proof.
   split; intros Γ' Δ ρ m ????; simpl;
     by rewrite (mem_unlock_all_spec (mem_unlock_all _)),
     !mem_locks_unlock_all, mem_unlock_empty.
 Qed.
-Lemma assert_unlock_impl Γ P Q : ((P → Q) ◊)%A ≡{Γ} (P ◊ → Q ◊)%A.
+Lemma assert_unlock_impl Γ δ P Q : ((P → Q) ◊)%A ≡{Γ,δ} (P ◊ → Q ◊)%A.
 Proof.
   split; [solve ltac:(eauto using mem_unlock_all_valid)|].
   solve ltac:(eauto using cmap_valid_weaken_squeeze, mem_unlock_memenv_of).
 Qed.
-Lemma assert_unlock_and Γ P Q : ((P ∧ Q) ◊)%A ≡{Γ} (P ◊ ∧ Q ◊)%A.
+Lemma assert_unlock_and Γ δ P Q : ((P ∧ Q) ◊)%A ≡{Γ,δ} (P ◊ ∧ Q ◊)%A.
 Proof. solve eauto. Qed.
-Lemma assert_unlock_or Γ P Q : ((P ∨ Q) ◊)%A ≡{Γ} (P ◊ ∨ Q ◊)%A.
+Lemma assert_unlock_or Γ δ P Q : ((P ∨ Q) ◊)%A ≡{Γ,δ} (P ◊ ∨ Q ◊)%A.
 Proof. solve eauto. Qed.
-Lemma assert_unlock_forall Γ {A} (P : A → assert K) :
-  ((∀ x, P x) ◊)%A ≡{Γ} (∀ x, (P x) ◊)%A.
+Lemma assert_unlock_forall Γ δ {A} (P : A → assert K) :
+  ((∀ x, P x) ◊)%A ≡{Γ,δ} (∀ x, (P x) ◊)%A.
 Proof. solve eauto. Qed.
-Lemma assert_unlock_exists Γ {A} (P : A → assert K) :
-  ((∃ x, P x) ◊)%A ≡{Γ} (∃ x, (P x) ◊)%A.
+Lemma assert_unlock_exists Γ δ {A} (P : A → assert K) :
+  ((∃ x, P x) ◊)%A ≡{Γ,δ} (∃ x, (P x) ◊)%A.
 Proof. solve eauto. Qed.
-Lemma assert_unlock_sep Γ P Q : (P ◊ ★ Q ◊)%A ⊆{Γ} ((P ★ Q) ◊)%A.
+Lemma assert_unlock_sep Γ δ P Q : (P ◊ ★ Q ◊)%A ⊆{Γ,δ} ((P ★ Q) ◊)%A.
 Proof.
-  intros Γ1 Δ1 ρ n m ???? (m1&m2&->&?&?&?).
+  intros Γ1 Δ δ1 ρ n m ?????? (m1&m2&->&?&?&?).
   exists (mem_unlock_all m1) (mem_unlock_all m2); split_ands; auto.
   * by rewrite mem_unlock_all_union by solve_sep_disjoint.
   * by rewrite <-!mem_unlock_all_disjoint_le.
 Qed.
-Lemma assert_unlock_sep_alt Γ P P' Q Q' :
-  P ⊆{Γ} (P' ◊)%A → Q ⊆{Γ} (Q' ◊)%A → (P ★ Q)%A ⊆{Γ} ((P' ★ Q') ◊)%A.
+Lemma assert_unlock_sep_alt Γ δ P P' Q Q' :
+  P ⊆{Γ,δ} (P' ◊)%A → Q ⊆{Γ,δ} (Q' ◊)%A → (P ★ Q)%A ⊆{Γ,δ} ((P' ★ Q') ◊)%A.
 Proof. intros HP HQ. by rewrite HP, HQ, assert_unlock_sep. Qed.
-Lemma assert_unlock_singleton Γ e1 e2 μ γ τ :
+Lemma assert_unlock_singleton Γ δ e1 e2 μ γ τ :
   perm_locked γ = true →
-  (e1 ↦{μ,γ} e2 : τ)%A ⊆{Γ} ((e1 ↦{μ,perm_unlock γ} e2 : τ) ◊)%A.
+  (e1 ↦{μ,γ} e2 : τ)%A ⊆{Γ,δ} ((e1 ↦{μ,perm_unlock γ} e2 : τ) ◊)%A.
 Proof.
-  intros ? Γ1 Δ1 ρ n m ???? (a&v&?&?&?&?&?).
+  intros ? Γ1 Δ δ1 ρ n m ?????? (a&v&?&?&?&?&?).
   exists a v; split_ands; eauto using mem_unlock_all_singleton.
 Qed.
-Lemma assert_unlock_singleton_ Γ e1 μ γ τ :
+Lemma assert_unlock_singleton_ Γ δ e1 μ γ τ :
   perm_locked γ = true →
-  (e1 ↦{μ,γ} - : τ)%A ⊆{Γ} ((e1 ↦{μ,perm_unlock γ} - : τ) ◊)%A.
+  (e1 ↦{μ,γ} - : τ)%A ⊆{Γ,δ} ((e1 ↦{μ,perm_unlock γ} - : τ) ◊)%A.
 Proof.
   intros Hγ. rewrite assert_unlock_exists.
-  by setoid_rewrite (λ e2, assert_unlock_singleton Γ e1 e2 μ γ τ Hγ).
+  by setoid_rewrite (λ e2, assert_unlock_singleton Γ δ e1 e2 μ γ τ Hγ).
 Qed.
-Lemma assert_lock_singleton Γ e1 e2 μ γ τ :
+Lemma assert_lock_singleton Γ δ e1 e2 μ γ τ :
   sep_valid γ → Some Writable ⊆ perm_kind γ →
-  (e1 ↦{μ,perm_lock γ} e2 : τ)%A ⊆{Γ} ((e1 ↦{μ,γ} e2 : τ) ◊)%A.
+  (e1 ↦{μ,perm_lock γ} e2 : τ)%A ⊆{Γ,δ} ((e1 ↦{μ,γ} e2 : τ) ◊)%A.
 Proof.
   intros. by rewrite assert_unlock_singleton,
     perm_unlock_lock by auto using perm_locked_lock.
 Qed.
-Lemma assert_lock_singleton_ Γ e1 μ γ τ :
+Lemma assert_lock_singleton_ Γ δ e1 μ γ τ :
   sep_valid γ → Some Writable ⊆ perm_kind γ →
-  (e1 ↦{μ,perm_lock γ} - : τ)%A ⊆{Γ} ((e1 ↦{μ,γ} - : τ) ◊)%A.
+  (e1 ↦{μ,perm_lock γ} - : τ)%A ⊆{Γ,δ} ((e1 ↦{μ,γ} - : τ) ◊)%A.
 Proof.
   intros. by rewrite assert_unlock_singleton_,
     perm_unlock_lock by auto using perm_locked_lock.
 Qed.
 
 Global Instance assert_unlock_unlock_indep P : UnlockIndep (P ◊).
-Proof. intros Γ. by rewrite assert_unlock_unlock. Qed.
+Proof. intros Γ δ. by rewrite assert_unlock_unlock. Qed.
 Global Instance assert_True_unlock_indep : UnlockIndep True.
 Proof. solve ltac:(eauto using mem_unlock_all_empty). Qed.
 Global Instance assert_False_unlock_indep : UnlockIndep False.
@@ -1095,11 +1113,11 @@ Global Instance assert_lift_unlock_indep : UnlockIndep P → UnlockIndep (P↑).
 Proof. solve ltac:(eauto using Forall_tail). Qed.
 Global Instance assert_sep_unlock_indep P Q :
   UnlockIndep P → UnlockIndep Q → UnlockIndep (P ★ Q).
-Proof. intros ?? Γ; auto using assert_unlock_sep_alt. Qed.
+Proof. intros ?? [Γ δ]; auto using assert_unlock_sep_alt. Qed.
 Global Instance assert_singleton_unlock_indep e1 e2 μ γ τ :
   perm_locked γ = false → UnlockIndep (e1 ↦{μ,γ} e2 : τ).
 Proof.
-  intros ? Γ Δ Γ' ρ n m ???? (a&v&?&?&?&?&?).
+  intros ? Γ δ Γ' Δ δ' ρ n m ?????? (a&v&?&?&?&?&?).
   exists a v; split_ands; eauto using mem_unlock_all_singleton_unlocked.
 Qed.
 End assertions.
