axiomatic_graph.v
@@ -4,29 +4,31 @@ Require Export restricted_smallstep memory_separation type_system.
 
 Record ax_frame_cond (K : Set) `{Env K} (A : Type) : Type := {
   frame :
-    env K → memenv K → ctx K → nat → focus K → mem K → mem K → A → Prop;
+    env K → memenv K → funenv K → ctx K → nat →
+    focus K → mem K → mem K → A → Prop;
   unframe :
-    env K → memenv K → ctx K → nat → focus K → mem K → mem K → A → Prop;
-  frame_valid Γ Δ k n φ m m' a :
-    ✓ Γ → frame Γ Δ k n φ m m' a → ✓{Γ,Δ} m → ✓{Γ,Δ} m';
-  unframe_valid Γ Δ k n φ m m' a :
-    ✓ Γ → unframe Γ Δ k n φ m m' a → ✓{Γ,Δ} m' → ✓{Γ,Δ} m
+    env K → memenv K → funenv K → ctx K → nat →
+    focus K → mem K → mem K → A → Prop;
+  frame_valid Γ Δ δ k n φ m m' a :
+    ✓ Γ → frame Γ Δ δ k n φ m m' a → ✓{Γ,Δ} m → ✓{Γ,Δ} m';
+  unframe_valid Γ Δ δ k n φ m m' a :
+    ✓ Γ → unframe Γ Δ δ k n φ m m' a → ✓{Γ,Δ} m' → ✓{Γ,Δ} m
 }.
-Arguments frame {_ _ _} _ _ _ _ _ _ _ _ _.
-Arguments unframe {_ _ _} _ _ _ _ _ _ _ _ _.
+Arguments frame {_ _ _} _ _ _ _ _ _ _ _ _ _.
+Arguments unframe {_ _ _} _ _ _ _ _ _ _ _ _ _.
 
 Record ax_assert (K : Set) `{Env K} : Type := {
   ax_assert_holds :
-    env K → memenv K → stack K → nat → focus K → mem K → Prop;
-  ax_assert_weaken Γ1 Γ2 Δ1 Δ2 ρ n n' φ m :
-    ✓ Γ1 → ✓{Γ1,Δ1} m → ✓{Δ1}* ρ →
-    ax_assert_holds Γ1 Δ1 ρ n φ m →
-    Γ1 ⊆ Γ2 → Δ1 ⇒ₘ Δ2 → n' ≤ n →
-    ax_assert_holds Γ2 Δ2 ρ n' φ m;
-  ax_assert_nf Γ δ Δ ρ n φ m m' :
-    ax_assert_holds Γ Δ ρ n φ m → nf (rcstep Γ δ ρ) (State [] φ m')
+    env K → memenv K → funenv K → stack K → nat → focus K → mem K → Prop;
+  ax_assert_weaken Γ1 Γ2 Δ1 Δ2 δ1 δ2 ρ n n' φ m :
+    ✓ Γ1 → ✓{Γ1,Δ1} δ1 → ✓{Γ1,Δ1} m → ✓{Δ1}* ρ →
+    ax_assert_holds Γ1 Δ1 δ1 ρ n φ m →
+    Γ1 ⊆ Γ2 → Δ1 ⇒ₘ Δ2 → δ1 ⊆ δ2 → n' ≤ n →
+    ax_assert_holds Γ2 Δ2 δ2 ρ n' φ m;
+  ax_assert_nf Γ Δ δ ρ n φ m m' :
+    ax_assert_holds Γ Δ δ ρ n φ m → nf (rcstep Γ δ ρ) (State [] φ m')
 }.
-Arguments ax_assert_holds {_ _} _ _ _ _ _ _ _.
+Arguments ax_assert_holds {_ _} _ _ _ _ _ _ _ _.
 Arguments ax_assert_nf {_ _} _ _ _ _ _ _ _ _ _ _ _.
 
 Section ax_graph.
@@ -48,22 +50,22 @@ Section basics.
        nat → ctx K → focus K → mem K → Prop :=
     | ax_O k φ m : ax_graph Δ ρ 0 k φ m
     | ax_done n φ m :
-       ax_assert_holds P Γ Δ ρ n φ m → ax_graph Δ ρ n [] φ m
+       ax_assert_holds P Γ Δ δ ρ n φ m → ax_graph Δ ρ n [] φ m
     | ax_further n k φ m :
        (∀ Δ' n' m' a,
          ✓{Γ,Δ'} m → Δ ⇒ₘ Δ' → n' < n →
-         frame F Γ Δ' k (S n') φ m m' a →
+         frame F Γ Δ' δ k (S n') φ m m' a →
          red (rcstep Γ δ ρ) (State k φ m')) →
        (∀ Δ' n' m' a S',
          ✓{Γ,Δ'} m → Δ ⇒ₘ Δ' → n' < n →
-         frame F Γ Δ' k (S n') φ m m' a →
+         frame F Γ Δ' δ k (S n') φ m m' a →
          Γ\ δ\ ρ ⊢ₛ State k φ m' ⇒ S' →
          dom indexset (SMem S') ∖ dom indexset m' ∩ dom indexset Δ' = ∅ →
          ax_next Δ' ρ n' a S') →
        ax_graph Δ ρ n k φ m
   with ax_next (Δ : memenv K) (ρ : stack K) : nat → A → state K → Prop :=
     | mk_ax_next Δ' k n φ m m' a :
-       unframe F Γ Δ' k (S n) φ m m' a →
+       unframe F Γ Δ' δ k (S n) φ m m' a →
        maybe Undef φ = None →
        focus_locks_valid φ m →
        ✓{Γ,Δ'} m' → Δ ⇒ₘ Δ' →
@@ -79,7 +81,7 @@ Section basics.
   Lemma ax_further_alt Δ ρ n k φ m :
     (∀ Δ' n' m' a,
       ✓{Γ,Δ'} m → Δ ⇒ₘ Δ' → n' < n →
-      frame F Γ Δ' k (S n') φ m m' a →
+      frame F Γ Δ' δ k (S n') φ m m' a →
       red (rcstep Γ δ ρ) (State k φ m') ∧
       ∀ S',
         Γ\ δ\ ρ ⊢ₛ State k φ m' ⇒ S' →
@@ -88,26 +90,26 @@ Section basics.
     ax_graph Δ ρ n k φ m.
   Proof. intros; apply ax_further; naive_solver. Qed.
   Lemma ax_graph_weaken Δ Δ' ρ n n' k φ m :
-    ✓ Γ → ✓{Γ,Δ} m → ✓{Δ}* ρ →
+    ✓ Γ → ✓{Γ,Δ} δ → ✓{Γ,Δ} m → ✓{Δ}* ρ →
     ax_graph Δ ρ n k φ m → Δ ⇒ₘ Δ' → n' ≤ n →
     ax_graph Δ' ρ n' k φ m.
   Proof.
-    intros ??? Hax ??. destruct Hax as [k φ m|n2 φ m|n2 k φ m Hred Hstep].
+    intros ???? Hax ??. destruct Hax as [k φ m|n2 φ m|n2 k φ m Hred Hstep].
     * replace n' with 0 by lia. constructor.
     * apply ax_done; eauto using ax_assert_weaken.
     * constructor; eauto with arith.
   Qed.
   Lemma ax_step Δ ρ n k φ m m' a S' :
-    ✓{Γ,Δ} m → frame F Γ Δ k (S n) φ m m' a →
+    ✓{Γ,Δ} m → frame F Γ Δ δ k (S n) φ m m' a →
     Γ\ δ\ ρ ⊢ₛ State k φ m' ⇒ S' →
     dom indexset (SMem S') ∖ dom indexset m' ∩ dom indexset Δ = ∅ →
     ax_graph Δ ρ (S n) k φ m → ax_next Δ ρ n a S'.
   Proof.
     inversion 5; subst; eauto.
-    destruct (ax_assert_nf P Γ δ Δ ρ (S n) φ m m'); eauto.
+    destruct (ax_assert_nf P Γ Δ δ ρ (S n) φ m m'); eauto.
   Qed.
   Lemma ax_step_undef Δ ρ n k φ m m' a k' Su m'' :
-    ✓{Γ,Δ} m → frame F Γ Δ k (S n) φ m m' a →
+    ✓{Γ,Δ} m → frame F Γ Δ δ k (S n) φ m m' a →
     Γ\ δ\ ρ ⊢ₛ State k φ m' ⇒ State k' (Undef Su) m'' →
     dom indexset m'' ∖ dom indexset m' ∩ dom indexset Δ = ∅ →
     ¬ax_graph Δ ρ (S n) k φ m.
@@ -116,8 +118,8 @@ Section basics.
     by feed inversion (ax_step Δ ρ n k φ m m' a (State k' (Undef Su) m'')).
   Qed.
   Lemma ax_red Δ ρ n k φ m m' a :
-    ✓{Γ,Δ} m → frame F Γ Δ k (S n) φ m m' a →
-    ¬ax_assert_holds P Γ Δ ρ (S n) φ m →
+    ✓{Γ,Δ} m → frame F Γ Δ δ k (S n) φ m m' a →
+    ¬ax_assert_holds P Γ Δ δ ρ (S n) φ m →
     ax_graph Δ ρ (S n) k φ m →
     red (rcstep Γ δ ρ) (State k φ m').
   Proof. by inversion 4; subst; eauto. Qed.
@@ -126,53 +128,54 @@ End basics.
 (** The predicate [ax] can be composed. This property is used to prove the
 structural Hoare rules. *)
 Definition ax_compose_diagram {A B} (F : ax_frame_cond K A)
-    (G : ax_frame_cond K B) (Γ : env K) (k2 : ctx K) := ∀ Δ k1 n φ m m' b,
-  ✓{Γ,Δ} m →
-  frame G Γ Δ (k1 ++ k2) n φ m m' b → ∃ a,
-  (**i 1.) *) frame F Γ Δ k1 n φ m m' a ∧
+    (G : ax_frame_cond K B) (Γ : env K) (k2 : ctx K) := ∀ Δ δ k1 n φ m m' b,
+  ✓{Γ,Δ} δ → ✓{Γ,Δ} m →
+  frame G Γ Δ δ (k1 ++ k2) n φ m m' b → ∃ a,
+  (**i 1.) *) frame F Γ Δ δ k1 n φ m m' a ∧
   (**i 2.) *) ∀ Δ' k1' φ' m2 m2',
     ✓{Γ,Δ'} m2' → Δ ⇒ₘ Δ' →
-    unframe F Γ Δ' k1' n φ' m2 m2' a →
-    unframe G Γ Δ' (k1' ++ k2) n φ' m2 m2' b.
+    unframe F Γ Δ' δ k1' n φ' m2 m2' a →
+    unframe G Γ Δ' δ (k1' ++ k2) n φ' m2 m2' b.
 Lemma ax_compose_diagram_diag {A} (F : ax_frame_cond K A) Γ :
   ax_compose_diagram F F Γ [].
 Proof.
-  intros Δ k1 n φ m m' a; rewrite (right_id_L [] (++)); exists a; split; auto.
+  intros Δ δ k1 n φ m m' a; rewrite (right_id_L [] (++)); exists a; split; auto.
   by intros; rewrite (right_id_L [] (++)).
 Qed.
 Lemma ax_compose {A B} (F : ax_frame_cond K A) (G : ax_frame_cond K B)
     (P Q : ax_assert K) Γ δ Δ n φ ρ k1 k2 m :
-  ✓ Γ →
+  ✓ Γ → ✓{Γ,Δ} δ →
   ax_compose_diagram F G Γ k2 →
   ✓{Γ,Δ} m →
   ax_graph F P Γ δ Δ (rlocals ρ k2) n k1 φ m →
   (∀ Δ' n' φ' m',
-    ax_assert_holds P Γ Δ' (rlocals ρ k2) n' φ' m' →
+    ax_assert_holds P Γ Δ' δ (rlocals ρ k2) n' φ' m' →
     ✓{Γ,Δ'} m' → Δ ⇒ₘ Δ' → n' ≤ n →
     ax_graph G Q Γ δ Δ' ρ n' k2 φ' m') →
   ax_graph G Q Γ δ Δ ρ n (k1 ++ k2) φ m.
 Proof.
   intros ?. revert Δ m k1 φ.
   induction n as [[|n] IH] using lt_wf_ind; [intros; apply ax_O|].
-  intros Δ m k1 φ HF ? Hax Hnext.
+  intros Δ m k1 φ ? HF ? Hax Hnext.
   inversion Hax as [| |???? Hred Hstep]; subst; eauto.
   apply ax_further_alt; intros Δ' n' m'' b ????.
-  destruct (HF Δ' k1 (S n') φ m m'' b) as (a&?&?); auto.
+  destruct (HF Δ' δ k1 (S n') φ m m'' b) as (a&?&?);
+    eauto using funenv_valid_weaken.
   split; [eauto using rcred_app|intros [k' φ' m'] p ?].
   destruct (cstep_app_suffix_of Γ δ ρ k1 k2 φ m'' (State k' φ' m'))
     as [k3 ?]; simplify_equality'; eauto.
   feed inversion (Hstep Δ' n' m'' a (State k3 φ' m'))
     as [Δ'' n'' k'' φ'' m2' m2 b']; subst; auto using rcstep_app_inv.
-  econstructor; eauto 10 using unframe_valid.
+  econstructor; eauto 10 using unframe_valid, funenv_valid_weaken.
 Qed.
 Lemma ax_compose_cons {A B} (F : ax_frame_cond K A) (G : ax_frame_cond K B)
     (P Q : ax_assert K) Γ δ Δ n φ ρ Ek m :
-  ✓ Γ →
+  ✓ Γ → ✓{Γ,Δ} δ →
   ax_compose_diagram F G Γ [Ek] →
   ✓{Γ,Δ} m →
   ax_graph F P Γ δ Δ (rlocals ρ [Ek]) n [] φ m →
   (∀ Δ' n' φ' m',
-    ax_assert_holds P Γ Δ' (rlocals ρ [Ek]) n' φ' m' →
+    ax_assert_holds P Γ Δ' δ (rlocals ρ [Ek]) n' φ' m' →
     ✓{Γ,Δ'} m' → Δ ⇒ₘ Δ' → n' ≤ n →
     ax_graph G Q Γ δ Δ' ρ n' [Ek] φ' m') →
   ax_graph G Q Γ δ Δ ρ n [Ek] φ m.
@@ -182,18 +185,18 @@ Proof. intros ?; by apply ax_compose. Qed.
 conjunction rule. These abstract versions are used to prove the concrete rules
 for both the expression and statement judgment. *)
 Definition ax_frame_diagram {A B} (F: ax_frame_cond K A) (G: ax_frame_cond K B)
-    (Γ : env K) (mf : mem K) := ∀ Δ k n φ m m' b,
-  ⊥ [m; mf] → ✓{Γ,Δ} m → ✓{Γ,Δ} mf →
-  frame G Γ Δ k n φ (m ∪ mf) m' b → ∃ a,
-  (**i 1.) *) frame F Γ Δ k n φ m m' a ∧
+    (Γ : env K) (mf : mem K) := ∀ Δ δ k n φ m m' b,
+  ✓{Γ,Δ} δ → ⊥ [m; mf] → ✓{Γ,Δ} m → ✓{Γ,Δ} mf →
+  frame G Γ Δ δ k n φ (m ∪ mf) m' b → ∃ a,
+  (**i 1.) *) frame F Γ Δ δ k n φ m m' a ∧
   (**i 2.) *) ∀ Δ' k' φ' m2 m2',
-    unframe F Γ Δ' k' n φ' m2 m2' a →
+    unframe F Γ Δ' δ k' n φ' m2 m2' a →
     ✓{Γ,Δ'} m2' → Δ ⇒ₘ Δ' →
-    unframe G Γ Δ' k' n φ' (m2 ∪ mf) m2' b ∧ ⊥ [m2; mf].
+    unframe G Γ Δ' δ k' n φ' (m2 ∪ mf) m2' b ∧ ⊥ [m2; mf].
 Lemma ax_frame_diagram_empty {A} (F : ax_frame_cond K A) Γ :
   ✓ Γ → ax_frame_diagram F F Γ ∅.
 Proof.
-  intros ??????? a ??? Ha; exists a.
+  intros ???????? a ???? Ha; exists a.
   rewrite sep_right_id in Ha by solve_sep_disjoint.
   split; auto; intros Δ' k' φ' m2 m2' ???.
   assert (sep_valid m2) by eauto using cmap_valid_sep_valid, unframe_valid.
@@ -201,78 +204,81 @@ Proof.
 Qed.
 Lemma ax_frame {A B}(F : ax_frame_cond K A) (G : ax_frame_cond K B)
     (P Q : ax_assert K) Γ δ Δ ρ n k φ m mf :
-  ✓ Γ →
+  ✓ Γ → ✓{Γ,Δ} δ →
   ax_frame_diagram F G Γ mf →
   ⊥ [m; mf] → ✓{Γ,Δ} m → ✓{Γ,Δ} mf →
   ax_graph F P Γ δ Δ ρ n k φ m →
   (∀ Δ' n' φ' m',
     ⊥ [m'; mf] → ✓{Γ,Δ'} m' → ✓{Γ,Δ'} mf → Δ ⇒ₘ Δ' → n' ≤ n →
-    ax_assert_holds P Γ Δ' ρ n' φ' m' →
-    ax_assert_holds Q Γ Δ' ρ n' φ' (m' ∪ mf)) →
+    ax_assert_holds P Γ Δ' δ ρ n' φ' m' →
+    ax_assert_holds Q Γ Δ' δ ρ n' φ' (m' ∪ mf)) →
   ax_graph G Q Γ δ Δ ρ n k φ (m ∪ mf).
 Proof.
-  intros ? HFG. revert Δ m k φ.
+  intros ? Hδ HFG. revert Δ m k φ Hδ.
   induction n as [[|n] IH] using lt_wf_ind; [intros; apply ax_O|].
-  intros Δ m k φ ??? Hax HPQ.
+  intros Δ m k φ ???? Hax HPQ.
   inversion Hax as [| |???? Hred Hstep]; subst; eauto using ax_done.
   apply ax_further_alt; intros Δ' n' m' a.
   rewrite cmap_union_valid by auto; intros [??] ???.
-  destruct (HFG Δ' k (S n') φ m m' a) as (b&?&Hunframe); eauto.
+  destruct (HFG Δ' δ k (S n') φ m m' a) as (b&?&Hunframe);
+    eauto using funenv_valid_weaken.
   split; [eauto|intros ? p ?].
   feed inversion (Hstep Δ' n' m' b S')
     as [Δ'' k' ? φ' m2' m2 ? τf']; subst; auto.
   destruct (Hunframe Δ'' k' φ' m2' m2 τf'); trivial.
-  apply mk_ax_next with Δ'' (m2' ∪ mf); eauto 10 using @cmap_valid_subseteq,
-    @sep_union_subseteq_r, unframe_valid, focus_locks_valid_union.
+  apply mk_ax_next with Δ'' (m2' ∪ mf);
+    eauto 11 using @cmap_valid_subseteq, @sep_union_subseteq_r,
+    unframe_valid, focus_locks_valid_union, funenv_valid_weaken.
 Qed.
 
 Lemma ax_weaken {A} (F G : ax_frame_cond K A)
     (P Q : ax_assert K) Γ δ Δ ρ n n' k φ m :
-  ✓ Γ → ✓{Γ,Δ} m → ✓{Δ}* ρ →
+  ✓ Γ → ✓{Γ,Δ} δ → ✓{Γ,Δ} m → ✓{Δ}* ρ →
   ax_graph F P Γ δ Δ ρ n k φ m →
   n' ≤ n →
   (∀ Δ' k' n' φ' m2 m2' a,
     ✓{Γ,Δ'} m2 →
-    frame G Γ Δ' k' n' φ' m2 m2' a →
+    frame G Γ Δ' δ k' n' φ' m2 m2' a →
     Δ ⇒ₘ Δ' → n' ≤ n →
-    frame F Γ Δ' k' n' φ' m2 m2' a) →
+    frame F Γ Δ' δ k' n' φ' m2 m2' a) →
   (∀ Δ' k' n' φ' m2 m2' a,
     ✓{Γ,Δ'} m2' →
-    unframe F Γ Δ' k' n' φ' m2 m2' a →
+    unframe F Γ Δ' δ k' n' φ' m2 m2' a →
     Δ ⇒ₘ Δ' → n' ≤ n →
-    unframe G Γ Δ' k' n' φ' m2 m2' a) →
+    unframe G Γ Δ' δ k' n' φ' m2 m2' a) →
   (∀ Δ' n' φ' m',
     ✓{Γ,Δ'} m' →
-    ax_assert_holds P Γ Δ' ρ n' φ' m' →
+    ax_assert_holds P Γ Δ' δ ρ n' φ' m' →
     Δ ⇒ₘ Δ' → n' ≤ n →
-    ax_assert_holds Q Γ Δ' ρ n' φ' m') →
+    ax_assert_holds Q Γ Δ' δ ρ n' φ' m') →
   ax_graph G Q Γ δ Δ ρ n' k φ m.
 Proof.
   intros ?; revert Δ k n' φ m.
-  induction n as [[|n] IH] using lt_wf_ind; intros Δ k n' φ m ?? Hax ????.
+  induction n as [[|n] IH] using lt_wf_ind; intros Δ k n' φ m ??? Hax ????.
   { replace n' with 0 by lia. by intros; apply ax_O. }
   inversion Hax as [| |???? Hred Hstep]; subst; eauto using ax_done.
-  { apply ax_done. eapply ax_assert_weaken with _ _ (S n); eauto. }
+  { apply ax_done. eapply ax_assert_weaken with _ _ _ (S n); eauto. }
   apply ax_further; eauto.
   { intros Δ' n'' m' a ????; eapply (Hred Δ' n'' m' a); eauto. }
   intros Δ' n'' m' a S' ???? p ?.
   feed inversion (Hstep Δ' n'' m' a S'); subst; eauto.
   econstructor; eauto.
-  eapply (IH n''); eauto using unframe_valid, indexes_valid_weaken.
+  eapply (IH n''); eauto using unframe_valid,
+    indexes_valid_weaken, funenv_valid_weaken.
 Qed.
 
 (** The standard framing condition that just adds an arbitrary frame to the
 memory before each step and takes it off after. *)
 Program Definition ax_disjoint_cond : ax_frame_cond K (mem K) := {|
-  frame Γ Δ k n φ m m' mf := m' = m ∪ mf ∧ ✓{Γ,Δ} mf ∧ ⊥ [m; mf];
-  unframe Γ Δ k n φ m m' mf := m' = m ∪ mf ∧ ⊥ [m; mf]
+  frame Γ Δ δ k n φ m m' mf := m' = m ∪ mf ∧ ✓{Γ,Δ} mf ∧ ⊥ [m; mf];
+  unframe Γ Δ δ k n φ m m' mf := m' = m ∪ mf ∧ ⊥ [m; mf]
 |}.
 Next Obligation. auto using cmap_union_valid_2. Qed.
 Next Obligation. eauto using cmap_valid_subseteq, @sep_union_subseteq_l. Qed.
 Lemma ax_disjoint_cond_frame_diagram Γ mf :
   ✓ Γ → ax_frame_diagram ax_disjoint_cond ax_disjoint_cond Γ mf.
 Proof.
-  intros ? Δ k n φ m m' mf' ??? (->&?&?). exists (mf ∪ mf'); split.
+  intros ? Δ δ k n φ m m' mf' ???? (->&?&?). exists (mf ∪ mf'); split.
   { split; split_ands; eauto using cmap_union_valid_2.
     by rewrite sep_associative by auto. }
   intros Δ' k' φ' m2 m2' [-> ?] ??; split; eauto.
@@ -281,6 +287,6 @@ Qed.
 Lemma ax_disjoint_compose_diagram Γ Ek :
   ax_compose_diagram ax_disjoint_cond ax_disjoint_cond Γ [Ek].
 Proof.
-  intros Δ k n φ m ? mf ? (->&?&?); exists mf; split_ands; eauto. by split.
+  intros Δ δ k n φ m ? mf ?? (->&?&?); exists mf; split_ands; eauto. by split.
 Qed.
 End ax_graph.
